workloads/Coq/BSTProplang/Runners/BespokeGenerator_test_runner.v
@@ -1,0 +1,41 @@
+From BSTProplang Require Import BespokeGenerator.
+From QuickChick Require Import QuickChick.
+Set Warnings "-extraction-opaque-accessed,-extraction".
+Axiom num_tests : nat. Extract Constant num_tests => "max_int".
+Definition qctest_test_prop_InsertValid_runner := (fun _ : unit => print_extracted_coq_string ("[|{" ++ show (withTime(fun tt => (sample1 test_prop_InsertValid_runner))) ++ "}|]")).
+Definition qctest_test_prop_DeleteValid_runner := (fun _ : unit => print_extracted_coq_string ("[|{" ++ show (withTime(fun tt => (sample1 test_prop_DeleteValid_runner))) ++ "}|]")).
+Definition qctest_test_prop_UnionValid_runner := (fun _ : unit => print_extracted_coq_string ("[|{" ++ show (withTime(fun tt => (sample1 test_prop_UnionValid_runner))) ++ "}|]")).
+Definition qctest_test_prop_InsertPost_runner := (fun _ : unit => print_extracted_coq_string ("[|{" ++ show (withTime(fun tt => (sample1 test_prop_InsertPost_runner))) ++ "}|]")).
+Definition qctest_test_prop_DeletePost_runner := (fun _ : unit => print_extracted_coq_string ("[|{" ++ show (withTime(fun tt => (sample1 test_prop_DeletePost_runner))) ++ "}|]")).
+Definition qctest_test_prop_UnionPost_runner := (fun _ : unit => print_extracted_coq_string ("[|{" ++ show (withTime(fun tt => (sample1 test_prop_UnionPost_runner))) ++ "}|]")).
+Definition qctest_test_prop_InsertModel_runner := (fun _ : unit => print_extracted_coq_string ("[|{" ++ show (withTime(fun tt => (sample1 test_prop_InsertModel_runner))) ++ "}|]")).
+Definition qctest_test_prop_DeleteModel_runner := (fun _ : unit => print_extracted_coq_string ("[|{" ++ show (withTime(fun tt => (sample1 test_prop_DeleteModel_runner))) ++ "}|]")).
+Definition qctest_test_prop_UnionModel_runner := (fun _ : unit => print_extracted_coq_string ("[|{" ++ show (withTime(fun tt => (sample1 test_prop_UnionModel_runner))) ++ "}|]")).
+Definition qctest_test_prop_InsertInsert_runner := (fun _ : unit => print_extracted_coq_string ("[|{" ++ show (withTime(fun tt => (sample1 test_prop_InsertInsert_runner))) ++ "}|]")).
+Definition qctest_test_prop_InsertDelete_runner := (fun _ : unit => print_extracted_coq_string ("[|{" ++ show (withTime(fun tt => (sample1 test_prop_InsertDelete_runner))) ++ "}|]")).
+Definition qctest_test_prop_InsertUnion_runner := (fun _ : unit => print_extracted_coq_string ("[|{" ++ show (withTime(fun tt => (sample1 test_prop_InsertUnion_runner))) ++ "}|]")).
+Definition qctest_test_prop_DeleteInsert_runner := (fun _ : unit => print_extracted_coq_string ("[|{" ++ show (withTime(fun tt => (sample1 test_prop_DeleteInsert_runner))) ++ "}|]")).
+Definition qctest_test_prop_DeleteDelete_runner := (fun _ : unit => print_extracted_coq_string ("[|{" ++ show (withTime(fun tt => (sample1 test_prop_DeleteDelete_runner))) ++ "}|]")).
+Definition qctest_test_prop_DeleteUnion_runner := (fun _ : unit => print_extracted_coq_string ("[|{" ++ show (withTime(fun tt => (sample1 test_prop_DeleteUnion_runner))) ++ "}|]")).
+Definition qctest_test_prop_UnionDeleteInsert_runner := (fun _ : unit => print_extracted_coq_string ("[|{" ++ show (withTime(fun tt => (sample1 test_prop_UnionDeleteInsert_runner))) ++ "}|]")).
+Definition qctest_test_prop_UnionUnionIdem_runner := (fun _ : unit => print_extracted_coq_string ("[|{" ++ show (withTime(fun tt => (sample1 test_prop_UnionUnionIdem_runner))) ++ "}|]")).
+Definition qctest_test_prop_UnionUnionAssoc_runner := (fun _ : unit => print_extracted_coq_string ("[|{" ++ show (withTime(fun tt => (sample1 test_prop_UnionUnionAssoc_runner))) ++ "}|]")).
+
+
+Parameter OCamlString : Type.
+Extract Constant OCamlString => "string".
+Axiom qctest_map : OCamlString -> unit.
+Extract Constant qctest_map => "
+fun test_name ->
+  let test_map = [
+    (""test_prop_InsertValid_runner"", qctest_test_prop_InsertValid_runner); (""test_prop_DeleteValid_runner"", qctest_test_prop_DeleteValid_runner); (""test_prop_UnionValid_runner"", qctest_test_prop_UnionValid_runner); (""test_prop_InsertPost_runner"", qctest_test_prop_InsertPost_runner); (""test_prop_DeletePost_runner"", qctest_test_prop_DeletePost_runner); (""test_prop_UnionPost_runner"", qctest_test_prop_UnionPost_runner); (""test_prop_InsertModel_runner"", qctest_test_prop_InsertModel_runner); (""test_prop_DeleteModel_runner"", qctest_test_prop_DeleteModel_runner); (""test_prop_UnionModel_runner"", qctest_test_prop_UnionModel_runner); (""test_prop_InsertInsert_runner"", qctest_test_prop_InsertInsert_runner); (""test_prop_InsertDelete_runner"", qctest_test_prop_InsertDelete_runner); (""test_prop_InsertUnion_runner"", qctest_test_prop_InsertUnion_runner); (""test_prop_DeleteInsert_runner"", qctest_test_prop_DeleteInsert_runner); (""test_prop_DeleteDelete_runner"", qctest_test_prop_DeleteDelete_runner); (""test_prop_DeleteUnion_runner"", qctest_test_prop_DeleteUnion_runner); (""test_prop_UnionDeleteInsert_runner"", qctest_test_prop_UnionDeleteInsert_runner); (""test_prop_UnionUnionIdem_runner"", qctest_test_prop_UnionUnionIdem_runner); (""test_prop_UnionUnionAssoc_runner"", qctest_test_prop_UnionUnionAssoc_runner)
+  ] in
+  let test = List.assoc test_name test_map in
+  test ()
+
+let () =
+Sys.argv.(1) |> qctest_map
+
+".
+
+Extraction "BespokeGenerator_test_runner.ml" qctest_test_prop_InsertValid_runner qctest_test_prop_DeleteValid_runner qctest_test_prop_UnionValid_runner qctest_test_prop_InsertPost_runner qctest_test_prop_DeletePost_runner qctest_test_prop_UnionPost_runner qctest_test_prop_InsertModel_runner qctest_test_prop_DeleteModel_runner qctest_test_prop_UnionModel_runner qctest_test_prop_InsertInsert_runner qctest_test_prop_InsertDelete_runner qctest_test_prop_InsertUnion_runner qctest_test_prop_DeleteInsert_runner qctest_test_prop_DeleteDelete_runner qctest_test_prop_DeleteUnion_runner qctest_test_prop_UnionDeleteInsert_runner qctest_test_prop_UnionUnionIdem_runner qctest_test_prop_UnionUnionAssoc_runner qctest_map.
