workloads/Coq/BSTProplang/Src/Impl.v
@@ -1,0 +1,156 @@
+
+Require Import List ZArith. Import ListNotations.
+Require Extraction.
+From QuickChick Require Import QuickChick.
+Import QcNotation.
+
+Inductive Tree :=
+| E 
+| T : Tree -> nat -> nat -> Tree -> Tree.
+
+Derive (Show) for Tree.
+
+
+Axiom fuel : nat. Extract Constant fuel => "100000".
+
+
+
+Fixpoint insert (k : nat) (v: nat) (t : Tree) :=
+  match t with
+  | E => T E k v E
+  | T l k' v' r => 
+  (*! *)                 
+    if k <? k' then T (insert k v l) k' v' r 
+    else if k' <? k then T l k' v' (insert k v r) 
+    else T l k' v r
+  (*!! insert_1  *)
+  (*!
+    T E k v E
+  *)
+  (*!! insert_2 *)
+(*!
+  if k <? k' then T (insert k v l) k' v' r
+  else T l k' v r *)
+ 
+  (*!! insert_3 *)
+  
+  (*! if k <? k' then T (insert k v l) k' v' r
+  else if k' <? k then T l k' v' (insert k v r)
+  else T l k' v' r *)
+ 
+  end.
+
+Fixpoint join (l: Tree) (r: Tree) :=
+  match l, r with
+  | E, _ => r
+  | _, E => l
+  | T l k v r, T l' k' v' r' =>
+    T l k v (T (join r l') k' v' r')
+  end
+.
+  
+
+Fixpoint delete (k: nat) (t: Tree) :=
+  match t with
+  | E => E
+  | T l k' v' r =>
+  (*! *)
+  if k <? k' then T (delete k l) k' v' r
+  else if k' <? k then T l k' v' (delete k r)
+  else join l r
+  (*!! delete_4 *)
+  (*!
+  if k <? k' then delete k l
+  else if k' <? k then delete k r
+  else join l r
+  *)
+  (*!! delete_5 *)
+  (*!
+  if k' <? k then T (delete k l) k' v' r
+  else if k <? k' then T l k' v' (delete k r)
+  else join l r
+  *)
+  end.
+
+
+
+Fixpoint below (k: nat) (t: Tree) :=
+  match k, t with
+  | _, E => E
+  | k, T l k' v r =>
+    if k <=? k' then below k l
+    else T l k' v (below k r)
+  end.
+
+Fixpoint above (k: nat) (t: Tree) :=
+  match k, t with
+  | _, E => E
+  | k, (T l k' v r) =>
+    if k' <=? k then above k r
+    else T (above k l) k' v r
+  end.
+
+
+
+
+Fixpoint union_ (l: Tree) (r: Tree) (f: nat) :=
+  match f with
+  | 0 => E
+  | S f' =>
+    match l, r with
+    | E, _ => r
+    | _, E => l
+    (*! *)
+    | (T l k v r), t =>
+      T (union_ l (below k t) f') k v (union_ r (above k t) f')
+    (*!! union_6 *)
+    (*!
+    | (T l k v r), (T l' k' v' r') =>
+      T l k v (T (union_ r l' f') k' v' r')
+    *)
+    (*!! union_7 *)
+    (*!     
+    | (T l k v r), (T l' k' v' r') =>
+      if k =? k' then T (union_ l l' f') k v (union_ r r' f')
+      else if k <? k' then T l k v (T (union_ r l' f') k' v' r')
+      else union_ (T l' k' v' r') (T l k v r) f'
+    *)
+    (*!! union_8 *)
+    (*!
+    | (T l k v r), (T l' k' v' r') =>
+    if k =? k'  then T (union_ l l' f') k v (union_ r r' f')
+    else if k <? k'   then T (union_ l (below k l') f') k v
+                            (union_ r (T (above k l') k' v' r') f')
+      else union_ (T l' k' v' r') (T l k v r) f' 
+    *)
+    end
+  end
+.
+
+Definition union (l: Tree) (r: Tree) :=
+  union_ l r fuel.
+
+
+Fixpoint find (k: nat) (t: Tree): option nat :=
+  match k, t with
+  | _, E => None
+  | k, (T l k' v' r) =>
+    if k <? k' then find k l
+    else if k' <? k then find k r
+    else Some v'
+  end
+.
+
+
+Fixpoint size (t: Tree) :=
+  match t with
+  | E => 0
+  | T l k v r => 1 + size l + size r
+  end
+.
+
+
+
+
+
+
