workloads/Coq/BSTProplang/Src/Spec.v
@@ -1,0 +1,218 @@
+
+From QuickChick Require Import QuickChick. Import QcNotation.
+From Coq Require Import Bool ZArith List. Import ListNotations.
+From BSTProplang Require Import Impl.
+
+Fixpoint keys (t: Tree): list nat :=
+  match t with
+  | E => nil
+  | T l k v r =>
+    let lk := keys l in
+    let rk := keys r in
+    [k] ++ lk ++ rk
+  end.
+
+
+Fixpoint all {A: Type} (f: A -> bool) (l: list A): bool :=
+  match l with
+  | nil => true
+  | (x::xs) =>
+      f x && all f xs
+  end
+  .
+
+
+Local Open Scope nat_scope.
+
+Definition Nat_gtb (n1 n2: nat) : bool :=
+  negb (n1 <=? n2).
+
+Fixpoint isBST (t: Tree): bool:=
+  match t with
+  | E => true
+  | (T l k _ r) =>
+    isBST l
+      && isBST r
+      && all (Nat_gtb k) (keys l)
+      && all (Nat.ltb k) (keys r)
+  end.
+
+
+
+
+Fixpoint toList (t: Tree): list (nat * nat) :=
+  match t with
+  | E => nil
+  | T l k v r =>
+    toList l ++ [(k, v)] ++ toList r
+  end.
+
+(* -- Validity properties. *)
+
+Definition prop_InsertValid (t: Tree) (k: nat) (v: nat) :=
+  isBST t -=> Some(isBST (insert k v t)).
+
+Definition prop_DeleteValid (t: Tree) (k: nat) :=
+  isBST t -=> Some(isBST (delete k t)).
+
+
+Definition prop_UnionValid (t1: Tree) (t2: Tree) :=
+  (isBST t1 && isBST t2) -=> (isBST (union t1 t2)).
+
+(* ---------- *)
+
+
+(* -- Postcondition properties. *)
+
+Definition prop_InsertPost (t: Tree) (k: nat) (k': nat) (v: nat) :=
+  isBST t
+    -=> (find k' (insert k v t) = if k =? k' then Some v else find k' t)?.
+
+Definition prop_DeletePost (t: Tree) (k: nat) (k': nat) :=
+  isBST t
+    -=> (find k' (delete k t) = if k =? k' then None else find k' t)?.
+
+Definition prop_UnionPost (t: Tree) (t': Tree) (k: nat) :=
+  isBST t
+    -=>
+    (let lhs := find k (union t t') in
+    match (find k t) with
+    | Some rhs => (lhs = (Some rhs))?
+    | None => match (find k t') with
+            | Some rhs => (lhs = (Some rhs))?
+            | None => (lhs = None)?
+            end
+    end).
+
+(* ---------- *)
+
+(* -- Model-based properties. *)
+
+Definition deleteKey  (k: nat) (l: list (nat * nat)): list (nat * nat) :=
+  filter (fun x => negb (fst x =? k)) l.
+
+Fixpoint L_insert (kv: nat * nat) (l: list (nat * nat)) : list (nat * nat) :=
+  match l with
+  | nil => [kv]
+  | (k, v)::xs =>
+    if fst kv =? k then (fst kv, snd kv)::xs
+    else if fst kv <? k then (fst kv, snd kv)::l
+    else (k, v)::(L_insert kv xs)
+  end.
+
+
+Fixpoint sorted (l: list (nat * nat)): bool :=
+  match l with
+  | nil => true
+  | (k, v)::l' =>
+    match l' with
+    | nil => true
+    | (k', v')::l'' =>
+      (k <? k') && sorted l'
+    end
+  end.
+
+
+Definition prop_InsertModel (t: Tree) (k: nat) (v: nat) :=
+  isBST t
+    -=> (toList (insert k v t) = L_insert (k, v) (deleteKey k (toList t)))?.
+
+
+Definition prop_DeleteModel (t: Tree) (k: nat) :=
+  isBST t
+    -=> Some((toList (delete k t) = deleteKey k (toList t))?).
+
+
+Fixpoint L_sort (l: list (nat * nat)): list (nat * nat) :=
+  match l with
+  | nil => nil
+  | (k, v)::l' =>
+    L_insert (k, v) (L_sort l')
+  end.
+
+Definition L_find (k: nat) (l: list (nat * nat)): option nat :=
+  match filter (fun x => fst x =? k) l with
+  | nil => None
+  | (k, v)::l' => Some v
+  end.
+
+Fixpoint L_unionBy (f: nat -> nat -> nat) (l1: list (nat * nat)) (l2: list (nat * nat)): list (nat * nat) :=
+  match l1 with
+  | nil => l2
+  | (k, v)::l1' =>
+    let l2' := deleteKey k l2 in
+    let v' := match L_find k l2 with
+              | None => v
+              | Some v' => f v v'
+              end
+    in
+    L_insert (k, v') (L_unionBy f l1' l2')
+  end.
+
+
+Definition prop_UnionModel (t: Tree) (t': Tree) :=
+  (isBST t && isBST t')
+    -=> (toList (union t t') = L_sort (L_unionBy (fun x y => x) (toList t) (toList t')))?.
+
+
+(* ---------- *)
+
+Fixpoint tree_eqb (t: Tree) (t': Tree) : bool :=
+  match t, t' with
+  | E, E => true
+  | T l k v r, T l' k' v' r' =>
+    (k =? k') && (v =? v') && tree_eqb l l' && tree_eqb r r'
+  | _, _ => false
+  end.
+
+
+Notation "A =|= B" := (tree_eqb A B) (at level 100, right associativity).
+(* -- Metamorphic properties. *)
+
+Definition prop_InsertInsert (t: Tree) (k: nat) (k': nat) (v: nat) (v': nat) :=
+  isBST t
+    -=> (insert k v (insert k' v' t) =|= if k =? k' then insert k v t else insert k' v' (insert k v t)).
+
+Definition prop_InsertDelete (t: Tree) (k: nat) (k': nat) (v: nat) :=
+  isBST t
+    -=> (insert k v (delete k' t) =|= if k =? k' then insert k v t else delete k' (insert k v t)).
+
+Definition prop_InsertUnion (t: Tree) (t': Tree) (k: nat) (v: nat) :=
+  (isBST t && isBST t')
+    -=> (insert k v (union t t') =|= union (insert k v t) t').
+
+Definition prop_DeleteInsert (t: Tree) (k: nat) (k': nat) (v': nat) :=
+  isBST t
+    -=>
+  (delete k (insert k' v' t) =|= if k =? k' then delete k t else insert k' v' (delete k t)).
+
+Definition prop_DeleteDelete (t: Tree) (k: nat) (k': nat) :=
+  isBST t
+    -=> (delete k (delete k' t) =|= delete k' (delete k t)).
+
+Definition prop_DeleteUnion (t: Tree) (t': Tree) (k: nat) :=
+  (isBST t && isBST t')
+    -=> Some(delete k (union t t')
+    =|= union (delete k t) (delete k t')).
+
+Definition prop_UnionDeleteInsert (t :Tree) (t': Tree) (k: nat) (v: nat) :=
+  (isBST t && isBST t')
+    -=> Some(union (delete k t) (insert k v t')
+    =|= insert k v (union t t')).
+
+Definition prop_UnionUnionIdem (t: Tree) :=
+  isBST t
+    -=> union t t =|= t.
+
+Definition prop_UnionUnionAssoc (t1: Tree) (t2: Tree) (t3: Tree) :=
+  (isBST t1 && isBST t2 && isBST t3)
+    -=> (union (union t1 t2) t3 =|= union t1 (union t2 t3)).
+
+
+
+(* ---------- *)
+
+Definition sizeBST (t: Tree) : nat :=
+  length (toList t).
+
+(* -- Size properties. *)
