workloads/Coq/BSTProplang/Strategies/BespokeFuzzer.v
@@ -1,0 +1,277 @@
+From QuickChick Require Import QuickChick.
+Import QcDefaultNotation. Open Scope qc_scope.
+Set Warnings "-extraction-opaque-accessed,-extraction".
+
+Require Import List ZArith.
+Import ListNotations.
+Import MonadNotation.
+
+From BSTProplang Require Import Impl.
+From BSTProplang Require Import Spec.
+From BSTProplang Require Import PropLang.
+
+Local Open Scope nat.
+Local Open Scope prop_scope.
+
+
+Fixpoint insert_correct (k : nat) (v: nat) (t : Tree) :=
+  match t with
+  | E => T E k v E
+  | T l k' v' r =>       
+    if k <? k' then T (insert k v l) k' v' r 
+    else if k' <? k then T l k' v' (insert k v r) 
+    else T l k' v r
+  end.
+
+
+Fixpoint gen_bst (s : nat) (lo hi : nat) : G Tree :=
+	let fix gen_bst (s : nat) (lo hi : nat) (t: Tree) : G Tree :=
+		match s with
+		| O => ret t
+		| S s' => 
+			if (lo <? hi) then	
+				k <- choose (lo, hi);;
+				v <- arbitrary;;
+				let t' := insert_correct k v t in
+				gen_bst s' lo hi t'
+			else
+				ret t
+		end
+	in
+	gen_bst s lo hi E.
+	
+
+Definition get_key (t : Tree) : option nat :=
+  match t with
+  | E => None
+  | T l k v r => Some k
+  end.
+
+Fixpoint mutate_bst_ (t : Tree) (lo hi: nat) : G Tree :=
+  match t with
+  | E => freq [(4, ret E)
+              ;(1, gen_bst 1 lo hi)]
+  | T l k v r => freq [	
+	(4, l' <- mutate_bst_ l lo (k - 1);; ret (T l' k v r));
+	(4, r' <- mutate_bst_ r (k + 1) hi;; ret (T l k v r'));
+    (2, 
+		let s := length (toList l) in
+		l' <- gen_bst s lo (k - 1);;
+		ret (T l' k v r));
+	(2, 
+		let s := length (toList r) in
+		r' <- gen_bst s (k + 1) hi;;
+		ret (T l k v r'));
+	(1, v' <- arbitrary;;
+		ret (T l k v' r))
+		]
+  end.
+
+#[local] Instance shrinkTree : Shrink Tree :=
+{|
+  shrink t := match t with
+              | E => []
+              | T l k v r => [l; r]
+              end
+|}.
+
+Definition bespoke := gen_bst 4 0 40.
+Definition mutate_bst := (fun t => mutate_bst_ t 0 40).
+
+Derive (Show) for Tree.
+
+Local Open Scope Z.
+
+#[local] Instance dec_eq_tree : Dec_Eq Tree.
+Proof. dec_eq. Defined.
+
+
+Axiom number_of_trials : nat.
+Extract Constant number_of_trials => "20000".
+
+Definition withInstrumentation' fn :=
+	let '(res, feedback) := withInstrumentation fn in
+	(res, Z.of_nat(snd feedback)).
+
+
+Definition test_prop_InsertValid   :=
+	@ForAll _ ∅ _ "t" (fun tt => bespoke) (fun tt n => (fun n => mutate_bst n)) (fun tt n => shrink n) (fun tt n => show n) (
+	@ForAll _ (Tree · ∅) _ "k" (fun '(t, tt) => arbitrary) (fun '(t, tt) n => (fun n => arbitrary)) (fun '(t, tt) n => shrink n) (fun '(t, tt) n => show n) (
+	@ForAll _ (nat · (Tree · ∅)) _ "v" (fun '(k, (t, tt)) => arbitrary) (fun '(k, (t, tt)) n => (fun n => arbitrary)) (fun '(k, (t, tt)) n => shrink n) (fun '(k, (t, tt)) n => show n) (
+	@Predicate (nat · (nat · (Tree · ∅))) Z
+	(fun '(v, (k, (t, tt))) => withInstrumentation' (fun _ => prop_InsertValid t k v))))).
+
+Definition test_prop_InsertValid_runner := (targetLoop number_of_trials test_prop_InsertValid (DynamicResettingSingletonPool.(mkPool) tt) DynamicResettingSingletonPool HillClimbingUtility).
+
+(*! QuickProp test_prop_InsertValid_runner. *)
+
+Definition test_prop_DeleteValid   :=
+	@ForAll _ ∅ _ "t" (fun tt => bespoke) (fun tt n => (fun n => mutate_bst n)) (fun tt n => shrink n) (fun tt n => show n) (
+	@ForAll _ (Tree · ∅) _ "k" (fun '(t, tt) => arbitrary) (fun '(t, tt) n => (fun n => arbitrary)) (fun '(t, tt) n => shrink n) (fun '(t, tt) n => show n) (
+	@Predicate (nat · (Tree · ∅)) Z
+	(fun '(k, (t, tt)) => withInstrumentation' (fun _ => prop_DeleteValid t k)))).
+
+Definition test_prop_DeleteValid_runner := (targetLoop number_of_trials test_prop_DeleteValid (DynamicResettingSingletonPool.(mkPool) tt) DynamicResettingSingletonPool HillClimbingUtility).
+(*! QuickProp test_prop_DeleteValid_runner. *)
+
+Definition test_prop_UnionValid    :=
+	@ForAll _ ∅ _ "t1" (fun tt => bespoke) (fun tt n => (fun n => mutate_bst n)) (fun tt n => shrink n) (fun tt n => show n) (
+	@ForAll _ (Tree · ∅) _ "t2" (fun '(t1, tt) => bespoke) (fun '(t1, tt) n => (fun n => mutate_bst n)) (fun '(t1, tt) n => shrink n) (fun '(t1, tt) n => show n) (
+	@Predicate (Tree · (Tree · ∅)) Z
+	(fun '(t2, (t1, tt)) => withInstrumentation' (fun _ => prop_UnionValid t1 t2)))).
+
+Definition test_prop_UnionValid_runner := (targetLoop number_of_trials test_prop_UnionValid (DynamicResettingSingletonPool.(mkPool) tt) DynamicResettingSingletonPool HillClimbingUtility).
+(*! QuickProp test_prop_UnionValid_runner. *)
+
+Definition test_prop_InsertPost    :=
+	@ForAll _ ∅ _ "t" (fun tt => bespoke) (fun tt n => (fun n => mutate_bst n)) (fun tt n => shrink n) (fun tt n => show n) (
+	@ForAll _ (Tree · ∅) _ "k" (fun '(t, tt) => arbitrary) (fun '(t, tt) n => (fun n => arbitrary)) (fun '(t, tt) n => shrink n) (fun '(t, tt) n => show n) (
+	@ForAll _ (nat · (Tree · ∅)) _ "k'" (fun '(k, (t, tt)) => arbitrary) (fun '(k, (t, tt)) n => (fun n => arbitrary)) (fun '(k, (t, tt)) n => shrink n) (fun '(k, (t, tt)) n => show n) (
+	@ForAll _ (nat · (nat · (Tree · ∅))) _ "v" (fun '(k', (k, (t, tt))) => arbitrary) (fun '(k', (k, (t, tt))) n => (fun n => arbitrary)) (fun '(k', (k, (t, tt))) n => shrink n) (fun '(k', (k, (t, tt))) n => show n) (
+	@Predicate (nat · (nat · (nat · (Tree · ∅)))) Z
+	(fun '(v, (k', (k, (t, tt)))) => withInstrumentation' (fun _ => prop_InsertPost t k k' v)))))).
+
+Definition test_prop_InsertPost_runner := (targetLoop number_of_trials test_prop_InsertPost (DynamicResettingSingletonPool.(mkPool) tt) DynamicResettingSingletonPool HillClimbingUtility).
+(*! QuickProp test_prop_InsertPost_runner. *)
+
+Definition test_prop_DeletePost    :=
+	@ForAll _ ∅ _ "t" (fun tt => bespoke) (fun tt n => (fun n => mutate_bst n)) (fun tt n => shrink n) (fun tt n => show n) (
+	@ForAll _ (Tree · ∅) _ "k" (fun '(t, tt) => arbitrary) (fun '(t, tt) n => (fun n => arbitrary)) (fun '(t, tt) n => shrink n) (fun '(t, tt) n => show n) (
+	@ForAll _ (nat · (Tree · ∅)) _ "k'" (fun '(k, (t, tt)) => arbitrary) (fun '(k, (t, tt)) n => (fun n => arbitrary)) (fun '(k, (t, tt)) n => shrink n) (fun '(k, (t, tt)) n => show n) (
+	@Predicate (nat · (nat · (Tree · ∅))) Z
+	(fun '(k', (k, (t, tt))) => withInstrumentation' (fun _ => prop_DeletePost t k k'))))).
+
+Definition test_prop_DeletePost_runner := (targetLoop number_of_trials test_prop_DeletePost (DynamicResettingSingletonPool.(mkPool) tt) DynamicResettingSingletonPool HillClimbingUtility).
+(*! QuickProp test_prop_DeletePost_runner. *)
+
+Definition test_prop_UnionPost   :=
+	@ForAll _ ∅ _ "t" (fun tt => bespoke) (fun tt n => (fun n => mutate_bst n)) (fun tt n => shrink n) (fun tt n => show n) (
+	@ForAll _ (Tree · ∅) _ "t'" (fun '(t, tt) => bespoke) (fun '(t, tt) n => (fun n => mutate_bst n)) (fun '(t, tt) n => shrink n) (fun '(t, tt) n => show n) (
+	@ForAll _ (Tree · (Tree · ∅)) _ "k" (fun '(t', (t, tt)) => arbitrary) (fun '(t', (t, tt)) n => (fun n => arbitrary)) (fun '(t', (t, tt)) n => shrink n) (fun '(t', (t, tt)) n => show n) (
+	@Predicate (nat · (Tree · (Tree · ∅))) Z
+	(fun '(k, (t', (t, tt))) => withInstrumentation' (fun _ => prop_UnionPost t t' k))))).
+
+Definition test_prop_UnionPost_runner := (targetLoop number_of_trials test_prop_UnionPost (DynamicResettingSingletonPool.(mkPool) tt) DynamicResettingSingletonPool HillClimbingUtility).
+(*! QuickProp test_prop_UnionPost_runner. *)
+
+Definition test_prop_InsertModel   :=
+	@ForAll _ ∅ _ "t" (fun tt => bespoke) (fun tt n => (fun n => mutate_bst n)) (fun tt n => shrink n) (fun tt n => show n) (
+	@ForAll _ (Tree · ∅) _ "k" (fun '(t, tt) => arbitrary) (fun '(t, tt) n => (fun n => arbitrary)) (fun '(t, tt) n => shrink n) (fun '(t, tt) n => show n) (
+	@ForAll _ (nat · (Tree · ∅)) _ "v" (fun '(k, (t, tt)) => arbitrary) (fun '(k, (t, tt)) n => (fun n => arbitrary)) (fun '(k, (t, tt)) n => shrink n) (fun '(k, (t, tt)) n => show n) (
+	@Predicate (nat · (nat · (Tree · ∅))) Z
+	(fun '(v, (k, (t, tt))) => withInstrumentation' (fun _ => prop_InsertModel t k v))))).
+
+Definition test_prop_InsertModel_runner := (targetLoop number_of_trials test_prop_InsertModel (DynamicResettingSingletonPool.(mkPool) tt) DynamicResettingSingletonPool HillClimbingUtility).
+(*! QuickProp test_prop_InsertModel_runner. *)
+
+Definition test_prop_DeleteModel   :=
+	@ForAll _ ∅ _ "t" (fun tt => bespoke) (fun tt n => (fun n => mutate_bst n)) (fun tt n => shrink n) (fun tt n => show n) (
+	@ForAll _ (Tree · ∅) _ "k" (fun '(t, tt) => arbitrary) (fun '(t, tt) n => (fun n => arbitrary)) (fun '(t, tt) n => shrink n) (fun '(t, tt) n => show n) (
+	@Predicate (nat · (Tree · ∅)) Z
+	(fun '(k, (t, tt)) => withInstrumentation' (fun _ => prop_DeleteModel t k)))).
+
+Definition test_prop_DeleteModel_runner := (targetLoop number_of_trials test_prop_DeleteModel (DynamicResettingSingletonPool.(mkPool) tt) DynamicResettingSingletonPool HillClimbingUtility).
+(*! QuickProp test_prop_DeleteModel_runner. *)
+
+Definition test_prop_UnionModel    :=
+	@ForAll _ ∅ _ "t" (fun tt => bespoke) (fun tt n => (fun n => mutate_bst n)) (fun tt n => shrink n) (fun tt n => show n) (
+	@ForAll _ (Tree · ∅) _ "t'" (fun '(t, tt) => bespoke) (fun '(t, tt) n => (fun n => mutate_bst n)) (fun '(t, tt) n => shrink n) (fun '(t, tt) n => show n) (
+	@Predicate (Tree · (Tree · ∅)) Z
+	(fun '(t', (t, tt)) => withInstrumentation' (fun _ => prop_UnionModel t t')))).
+
+Definition test_prop_UnionModel_runner := (targetLoop number_of_trials test_prop_UnionModel (DynamicResettingSingletonPool.(mkPool) tt) DynamicResettingSingletonPool HillClimbingUtility).
+(*! QuickProp test_prop_UnionModel_runner. *)
+
+Definition test_prop_InsertInsert    :=
+	@ForAll _ ∅ _ "t" (fun tt => bespoke) (fun tt n => (fun n => mutate_bst n)) (fun tt n => shrink n) (fun tt n => show n) (
+	@ForAll _ (Tree · ∅) _ "k" (fun '(t, tt) => arbitrary) (fun '(t, tt) n => (fun n => arbitrary)) (fun '(t, tt) n => shrink n) (fun '(t, tt) n => show n) (
+	@ForAll _ (nat · (Tree · ∅)) _ "k'" (fun '(k, (t, tt)) => arbitrary) (fun '(k, (t, tt)) n => (fun n => arbitrary)) (fun '(k, (t, tt)) n => shrink n) (fun '(k, (t, tt)) n => show n) (
+	@ForAll _ (nat · (nat · (Tree · ∅))) _ "v" (fun '(k', (k, (t, tt))) => arbitrary) (fun '(k', (k, (t, tt))) n => (fun n => arbitrary)) (fun '(k', (k, (t, tt))) n => shrink n) (fun '(k', (k, (t, tt))) n => show n) (
+	@ForAll _ (nat · (nat · (nat · (Tree · ∅)))) _ "v'" (fun '(v, (k', (k, (t, tt)))) => arbitrary) (fun '(v, (k', (k, (t, tt)))) n => (fun n => arbitrary)) (fun '(v, (k', (k, (t, tt)))) n => shrink n) (fun '(v, (k', (k, (t, tt)))) n => show n) (
+	@Predicate (nat · (nat · (nat · (nat · (Tree · ∅))))) Z
+	(fun '(v', (v, (k', (k, (t, tt))))) => withInstrumentation' (fun _ => prop_InsertInsert t k k' v v'))))))).
+
+Definition test_prop_InsertInsert_runner := (targetLoop number_of_trials test_prop_InsertInsert (DynamicResettingSingletonPool.(mkPool) tt) DynamicResettingSingletonPool HillClimbingUtility).
+(*! QuickProp test_prop_InsertInsert_runner. *)
+
+Definition test_prop_InsertDelete    :=
+	@ForAll _ ∅ _ "t" (fun tt => bespoke) (fun tt n => (fun n => mutate_bst n)) (fun tt n => shrink n) (fun tt n => show n) (
+	@ForAll _ (Tree · ∅) _ "k" (fun '(t, tt) => arbitrary) (fun '(t, tt) n => (fun n => arbitrary)) (fun '(t, tt) n => shrink n) (fun '(t, tt) n => show n) (
+	@ForAll _ (nat · (Tree · ∅)) _ "k'" (fun '(k, (t, tt)) => arbitrary) (fun '(k, (t, tt)) n => (fun n => arbitrary)) (fun '(k, (t, tt)) n => shrink n) (fun '(k, (t, tt)) n => show n) (
+	@ForAll _ (nat · (nat · (Tree · ∅))) _ "v" (fun '(k', (k, (t, tt))) => arbitrary) (fun '(k', (k, (t, tt))) n => (fun n => arbitrary)) (fun '(k', (k, (t, tt))) n => shrink n) (fun '(k', (k, (t, tt))) n => show n) (
+	@Predicate (nat · (nat · (nat · (Tree · ∅)))) Z
+	(fun '(v, (k', (k, (t, tt)))) => withInstrumentation' (fun _ => prop_InsertDelete t k k' v)))))).
+
+Definition test_prop_InsertDelete_runner := (targetLoop number_of_trials test_prop_InsertDelete (DynamicResettingSingletonPool.(mkPool) tt) DynamicResettingSingletonPool HillClimbingUtility).
+(*! QuickProp test_prop_InsertDelete_runner. *)
+
+Definition test_prop_InsertUnion   :=
+	@ForAll _ ∅ _ "t" (fun tt => bespoke) (fun tt n => (fun n => mutate_bst n)) (fun tt n => shrink n) (fun tt n => show n) (
+	@ForAll _ (Tree · ∅) _ "t'" (fun '(t, tt) => bespoke) (fun '(t, tt) n => (fun n => mutate_bst n)) (fun '(t, tt) n => shrink n) (fun '(t, tt) n => show n) (
+	@ForAll _ (Tree · (Tree · ∅)) _ "k" (fun '(t', (t, tt)) => arbitrary) (fun '(t', (t, tt)) n => (fun n => arbitrary)) (fun '(t', (t, tt)) n => shrink n) (fun '(t', (t, tt)) n => show n) (
+	@ForAll _ (nat · (Tree · (Tree · ∅))) _ "v" (fun '(k, (t', (t, tt))) => arbitrary) (fun '(k, (t', (t, tt))) n => (fun n => arbitrary)) (fun '(k, (t', (t, tt))) n => shrink n) (fun '(k, (t', (t, tt))) n => show n) (
+	@Predicate (nat · (nat · (Tree · (Tree · ∅)))) Z
+	(fun '(v, (k, (t', (t, tt)))) => withInstrumentation' (fun _ => prop_InsertUnion t t' k v)))))).
+
+Definition test_prop_InsertUnion_runner := (targetLoop number_of_trials test_prop_InsertUnion (DynamicResettingSingletonPool.(mkPool) tt) DynamicResettingSingletonPool HillClimbingUtility).
+(*! QuickProp test_prop_InsertUnion_runner. *)
+
+Definition test_prop_DeleteInsert    :=
+	@ForAll _ ∅ _ "t" (fun tt => bespoke) (fun tt n => (fun n => mutate_bst n)) (fun tt n => shrink n) (fun tt n => show n) (
+	@ForAll _ (Tree · ∅) _ "k" (fun '(t, tt) => arbitrary) (fun '(t, tt) n => (fun n => arbitrary)) (fun '(t, tt) n => shrink n) (fun '(t, tt) n => show n) (
+	@ForAll _ (nat · (Tree · ∅)) _ "k'" (fun '(k, (t, tt)) => arbitrary) (fun '(k, (t, tt)) n => (fun n => arbitrary)) (fun '(k, (t, tt)) n => shrink n) (fun '(k, (t, tt)) n => show n) (
+	@ForAll _ (nat · (nat · (Tree · ∅))) _ "v'" (fun '(k', (k, (t, tt))) => arbitrary) (fun '(k', (k, (t, tt))) n => (fun n => arbitrary)) (fun '(k', (k, (t, tt))) n => shrink n) (fun '(k', (k, (t, tt))) n => show n) (
+	@Predicate (nat · (nat · (nat · (Tree · ∅)))) Z
+	(fun '(v', (k', (k, (t, tt)))) => withInstrumentation' (fun _ => prop_DeleteInsert t k k' v')))))).
+
+Definition test_prop_DeleteInsert_runner := (targetLoop number_of_trials test_prop_DeleteInsert (DynamicResettingSingletonPool.(mkPool) tt) DynamicResettingSingletonPool HillClimbingUtility).
+(*! QuickProp test_prop_DeleteInsert_runner. *)
+
+Definition test_prop_DeleteDelete    :=
+	@ForAll _ ∅ _ "t" (fun tt => bespoke) (fun tt n => (fun n => mutate_bst n)) (fun tt n => shrink n) (fun tt n => show n) (
+	@ForAll _ (Tree · ∅) _ "k" (fun '(t, tt) => arbitrary) (fun '(t, tt) n => (fun n => arbitrary)) (fun '(t, tt) n => shrink n) (fun '(t, tt) n => show n) (
+	@ForAll _ (nat · (Tree · ∅)) _ "k'" (fun '(k, (t, tt)) => arbitrary) (fun '(k, (t, tt)) n => (fun n => arbitrary)) (fun '(k, (t, tt)) n => shrink n) (fun '(k, (t, tt)) n => show n) (
+	@Predicate (nat · (nat · (Tree · ∅))) Z
+	(fun '(k', (k, (t, tt))) => (withInstrumentation' (fun _ => prop_DeleteDelete t k k')))))).
+
+Definition test_prop_DeleteDelete_runner := (targetLoop number_of_trials test_prop_DeleteDelete (DynamicResettingSingletonPool.(mkPool) tt) DynamicResettingSingletonPool HillClimbingUtility).
+(*! QuickProp test_prop_DeleteDelete_runner. *)
+
+Definition test_prop_DeleteUnion   :=
+	@ForAll _ ∅ _ "t" (fun tt => bespoke) (fun tt n => (fun n => mutate_bst n)) (fun tt n => shrink n) (fun tt n => show n) (
+	@ForAll _ (Tree · ∅) _ "t'" (fun '(t, tt) => bespoke) (fun '(t, tt) n => (fun n => mutate_bst n)) (fun '(t, tt) n => shrink n) (fun '(t, tt) n => show n) (
+	@ForAll _ (Tree · (Tree · ∅)) _ "k" (fun '(t', (t, tt)) => arbitrary) (fun '(t', (t, tt)) n => (fun n => arbitrary)) (fun '(t', (t, tt)) n => shrink n) (fun '(t', (t, tt)) n => show n) (
+	@Predicate (nat · (Tree · (Tree · ∅))) Z
+	(fun '(k, (t', (t, tt))) => withInstrumentation' (fun _ => prop_DeleteUnion t t' k))))).
+
+Definition test_prop_DeleteUnion_runner := (targetLoop number_of_trials test_prop_DeleteUnion (DynamicResettingSingletonPool.(mkPool) tt) DynamicResettingSingletonPool HillClimbingUtility).
+(*! QuickProp test_prop_DeleteUnion_runner. *)
+
+Definition test_prop_UnionDeleteInsert   :=
+	@ForAll _ ∅ _ "t " (fun tt => bespoke) (fun tt n => (fun n => mutate_bst n)) (fun tt n => shrink n) (fun tt n => show n) (
+	@ForAll _ (Tree · ∅) _ "t'" (fun '(t , tt) => bespoke) (fun '(t , tt) n => (fun n => mutate_bst n)) (fun '(t , tt) n => shrink n) (fun '(t , tt) n => show n) (
+	@ForAll _ (Tree · (Tree · ∅)) _ "k" (fun '(t', (t , tt)) => arbitrary) (fun '(t', (t , tt)) n => (fun n => arbitrary)) (fun '(t', (t , tt)) n => shrink n) (fun '(t', (t , tt)) n => show n) (
+	@ForAll _ (nat · (Tree · (Tree · ∅))) _ "v" (fun '(k, (t', (t , tt))) => arbitrary) (fun '(k, (t', (t , tt))) n => (fun n => arbitrary)) (fun '(k, (t', (t , tt))) n => shrink n) (fun '(k, (t', (t , tt))) n => show n) (
+	@Predicate (nat · (nat · (Tree · (Tree · ∅)))) Z
+	(fun '(v, (k, (t', (t, tt)))) => (withInstrumentation' (fun _ => prop_UnionDeleteInsert t t' k v))))))).
+
+Definition test_prop_UnionDeleteInsert_runner := (targetLoop number_of_trials test_prop_UnionDeleteInsert (DynamicResettingSingletonPool.(mkPool) tt) DynamicResettingSingletonPool HillClimbingUtility).
+(*! QuickProp test_prop_UnionDeleteInsert_runner. *)
+
+Definition test_prop_UnionUnionIdem    :=
+	@ForAll _ ∅ _ "t" (fun tt => bespoke) (fun tt n => (fun n => mutate_bst n)) (fun tt n => shrink n) (fun tt n => show n) (
+	@Predicate (Tree · ∅) Z
+	(fun '(t, tt) => withInstrumentation' (fun _ => prop_UnionUnionIdem t))).
+
+Definition test_prop_UnionUnionIdem_runner := (targetLoop number_of_trials test_prop_UnionUnionIdem (DynamicResettingSingletonPool.(mkPool) tt) DynamicResettingSingletonPool HillClimbingUtility).
+(*! QuickProp test_prop_UnionUnionIdem_runner. *)
+
+Definition test_prop_UnionUnionAssoc   :=
+	@ForAll _ ∅ _ "t1" (fun tt => bespoke) (fun tt n => (fun n => mutate_bst n)) (fun tt n => shrink n) (fun tt n => show n) (
+	@ForAll _ (Tree · ∅) _ "t2" (fun '(t1, tt) => bespoke) (fun '(t1, tt) n => (fun n => mutate_bst n)) (fun '(t1, tt) n => shrink n) (fun '(t1, tt) n => show n) (
+	@ForAll _ (Tree · (Tree · ∅)) _ "t3" (fun '(t2, (t1, tt)) => bespoke) (fun '(t2, (t1, tt)) n => (fun n => mutate_bst n)) (fun '(t2, (t1, tt)) n => shrink n) (fun '(t2, (t1, tt)) n => show n) (
+	@Predicate (Tree · (Tree · (Tree · ∅))) Z
+	(fun '(t3, (t2, (t1, tt))) => withInstrumentation' (fun _ => prop_UnionUnionAssoc t1 t2 t3))))).
+
+Definition test_prop_UnionUnionAssoc_runner := (targetLoop number_of_trials test_prop_UnionUnionAssoc (DynamicResettingSingletonPool.(mkPool) tt) DynamicResettingSingletonPool HillClimbingUtility).
+(*! QuickProp test_prop_UnionUnionAssoc_runner. *)
