workloads/Coq/BSTProplang/Strategies/SpecificationBasedGenerator.v
@@ -1,0 +1,236 @@
+From QuickChick Require Import QuickChick.
+Import QcDefaultNotation. Open Scope qc_scope.
+Set Warnings "-extraction-opaque-accessed,-extraction".
+
+Require Import List ZArith.
+Import ListNotations.
+Import MonadNotation.
+
+From BSTProplang Require Import Impl.
+From BSTProplang Require Import Spec.
+From BSTProplang Require Import PropLang.
+
+Local Open Scope nat.
+Local Open Scope prop_scope.
+
+
+Inductive between : nat -> nat -> nat -> Prop :=
+| between_n : forall n m, le n m -> between n (S n) (S (S m))
+| between_S : forall n m o, between n m o -> between n (S m) (S o).
+
+Derive DecOpt for (le x y).
+Derive ArbitrarySizedSuchThat for (fun x => le y x).
+
+Derive ArbitrarySizedSuchThat for (fun x => between lo x hi).
+Derive DecOpt for (between lo x hi).
+
+Inductive bst : nat -> nat -> Tree -> Prop :=
+| bst_leaf : forall lo hi, bst lo hi E
+| bst_node : forall lo hi k v l r,
+    between lo k hi ->
+    bst lo k l -> bst k hi r ->
+    bst lo hi (T l k v r).
+
+Derive ArbitrarySizedSuchThat for (fun t => bst lo hi t).
+Derive DecOpt for (bst lo hi t).
+
+#[local] Instance shrinkTree : Shrink Tree :=
+{|
+  shrink t := match t with
+              | E => []
+              | T l k v r => [l; r]
+              end
+|}.
+
+Definition spec_derived := (@arbitrarySizeST _ (fun t => bst 0 100 t) _ 10).
+Derive (Show) for Tree.
+
+Local Open Scope Z.
+
+#[local] Instance dec_eq_tree : Dec_Eq Tree.
+Proof. dec_eq. Defined.
+
+Axiom number_of_trials : nat.
+Extract Constant number_of_trials => "20000".
+
+Definition test_prop_InsertValid   :=
+	@ForAllMaybe _ ∅ _ "t" (fun tt => spec_derived) (fun tt n => (fun n => spec_derived)) (fun tt n => shrink n) (fun tt n => show n) (
+	@ForAll _ (Tree · ∅) _ "k" (fun '(t, tt) => arbitrary) (fun '(t, tt) n => (fun n => arbitrary)) (fun '(t, tt) n => shrink n) (fun '(t, tt) n => show n) (
+	@ForAll _ (nat · (Tree · ∅)) _ "v" (fun '(k, (t, tt)) => arbitrary) (fun '(k, (t, tt)) n => (fun n => arbitrary)) (fun '(k, (t, tt)) n => shrink n) (fun '(k, (t, tt)) n => show n) (
+	@Predicate (nat · (nat · (Tree · ∅))) Z
+	(fun '(v, (k, (t, tt))) => (prop_InsertValid t k v, 0%Z))))).
+
+Definition test_prop_InsertValid_runner := (targetLoop number_of_trials test_prop_InsertValid (DynamicResettingSingletonPool.(mkPool) tt) DynamicResettingSingletonPool HillClimbingUtility).
+
+(*! QuickProp test_prop_InsertValid_runner. *)
+
+Definition test_prop_DeleteValid   :=
+	@ForAllMaybe _ ∅ _ "t" (fun tt => spec_derived) (fun tt n => (fun n => spec_derived)) (fun tt n => shrink n) (fun tt n => show n) (
+	@ForAll _ (Tree · ∅) _ "k" (fun '(t, tt) => arbitrary) (fun '(t, tt) n => (fun n => arbitrary)) (fun '(t, tt) n => shrink n) (fun '(t, tt) n => show n) (
+	@Predicate (nat · (Tree · ∅)) Z
+	(fun '(k, (t, tt)) => (prop_DeleteValid t k, 0%Z)))).
+
+Definition test_prop_DeleteValid_runner := (targetLoop number_of_trials test_prop_DeleteValid (DynamicResettingSingletonPool.(mkPool) tt) DynamicResettingSingletonPool HillClimbingUtility).
+(*! QuickProp test_prop_DeleteValid_runner. *)
+
+Definition test_prop_UnionValid    :=
+	@ForAllMaybe _ ∅ _ "t1" (fun tt => spec_derived) (fun tt n => (fun n => spec_derived)) (fun tt n => shrink n) (fun tt n => show n) (
+	@ForAllMaybe _ (Tree · ∅) _ "t2" (fun '(t1, tt) => spec_derived) (fun '(t1, tt) n => (fun n => spec_derived)) (fun '(t1, tt) n => shrink n) (fun '(t1, tt) n => show n) (
+	@Predicate (Tree · (Tree · ∅)) Z
+	(fun '(t2, (t1, tt)) => (prop_UnionValid t1 t2, 0%Z)))).
+
+Definition test_prop_UnionValid_runner := (targetLoop number_of_trials test_prop_UnionValid (DynamicResettingSingletonPool.(mkPool) tt) DynamicResettingSingletonPool HillClimbingUtility).
+(*! QuickProp test_prop_UnionValid_runner. *)
+
+Definition test_prop_InsertPost    :=
+	@ForAllMaybe _ ∅ _ "t" (fun tt => spec_derived) (fun tt n => (fun n => spec_derived)) (fun tt n => shrink n) (fun tt n => show n) (
+	@ForAll _ (Tree · ∅) _ "k" (fun '(t, tt) => arbitrary) (fun '(t, tt) n => (fun n => arbitrary)) (fun '(t, tt) n => shrink n) (fun '(t, tt) n => show n) (
+	@ForAll _ (nat · (Tree · ∅)) _ "k'" (fun '(k, (t, tt)) => arbitrary) (fun '(k, (t, tt)) n => (fun n => arbitrary)) (fun '(k, (t, tt)) n => shrink n) (fun '(k, (t, tt)) n => show n) (
+	@ForAll _ (nat · (nat · (Tree · ∅))) _ "v" (fun '(k', (k, (t, tt))) => arbitrary) (fun '(k', (k, (t, tt))) n => (fun n => arbitrary)) (fun '(k', (k, (t, tt))) n => shrink n) (fun '(k', (k, (t, tt))) n => show n) (
+	@Predicate (nat · (nat · (nat · (Tree · ∅)))) Z
+	(fun '(v, (k', (k, (t, tt)))) => (prop_InsertPost t k k' v, 0%Z)))))).
+
+Definition test_prop_InsertPost_runner := (targetLoop number_of_trials test_prop_InsertPost (DynamicResettingSingletonPool.(mkPool) tt) DynamicResettingSingletonPool HillClimbingUtility).
+(*! QuickProp test_prop_InsertPost_runner. *)
+
+Definition test_prop_DeletePost    :=
+	@ForAllMaybe _ ∅ _ "t" (fun tt => spec_derived) (fun tt n => (fun n => spec_derived)) (fun tt n => shrink n) (fun tt n => show n) (
+	@ForAll _ (Tree · ∅) _ "k" (fun '(t, tt) => arbitrary) (fun '(t, tt) n => (fun n => arbitrary)) (fun '(t, tt) n => shrink n) (fun '(t, tt) n => show n) (
+	@ForAll _ (nat · (Tree · ∅)) _ "k'" (fun '(k, (t, tt)) => arbitrary) (fun '(k, (t, tt)) n => (fun n => arbitrary)) (fun '(k, (t, tt)) n => shrink n) (fun '(k, (t, tt)) n => show n) (
+	@Predicate (nat · (nat · (Tree · ∅))) Z
+	(fun '(k', (k, (t, tt))) => (prop_DeletePost t k k', 0%Z))))).
+
+Definition test_prop_DeletePost_runner := (targetLoop number_of_trials test_prop_DeletePost (DynamicResettingSingletonPool.(mkPool) tt) DynamicResettingSingletonPool HillClimbingUtility).
+(*! QuickProp test_prop_DeletePost_runner. *)
+
+Definition test_prop_UnionPost   :=
+	@ForAllMaybe _ ∅ _ "t" (fun tt => spec_derived) (fun tt n => (fun n => spec_derived)) (fun tt n => shrink n) (fun tt n => show n) (
+	@ForAllMaybe _ (Tree · ∅) _ "t'" (fun '(t, tt) => spec_derived) (fun '(t, tt) n => (fun n => spec_derived)) (fun '(t, tt) n => shrink n) (fun '(t, tt) n => show n) (
+	@ForAll _ (Tree · (Tree · ∅)) _ "k" (fun '(t', (t, tt)) => arbitrary) (fun '(t', (t, tt)) n => (fun n => arbitrary)) (fun '(t', (t, tt)) n => shrink n) (fun '(t', (t, tt)) n => show n) (
+	@Predicate (nat · (Tree · (Tree · ∅))) Z
+	(fun '(k, (t', (t, tt))) => (prop_UnionPost t t' k, 0%Z))))).
+
+Definition test_prop_UnionPost_runner := (targetLoop number_of_trials test_prop_UnionPost (DynamicResettingSingletonPool.(mkPool) tt) DynamicResettingSingletonPool HillClimbingUtility).
+(*! QuickProp test_prop_UnionPost_runner. *)
+
+Definition test_prop_InsertModel   :=
+	@ForAllMaybe _ ∅ _ "t" (fun tt => spec_derived) (fun tt n => (fun n => spec_derived)) (fun tt n => shrink n) (fun tt n => show n) (
+	@ForAll _ (Tree · ∅) _ "k" (fun '(t, tt) => arbitrary) (fun '(t, tt) n => (fun n => arbitrary)) (fun '(t, tt) n => shrink n) (fun '(t, tt) n => show n) (
+	@ForAll _ (nat · (Tree · ∅)) _ "v" (fun '(k, (t, tt)) => arbitrary) (fun '(k, (t, tt)) n => (fun n => arbitrary)) (fun '(k, (t, tt)) n => shrink n) (fun '(k, (t, tt)) n => show n) (
+	@Predicate (nat · (nat · (Tree · ∅))) Z
+	(fun '(v, (k, (t, tt))) => (prop_InsertModel t k v, 0%Z))))).
+
+Definition test_prop_InsertModel_runner := (targetLoop number_of_trials test_prop_InsertModel (DynamicResettingSingletonPool.(mkPool) tt) DynamicResettingSingletonPool HillClimbingUtility).
+(*! QuickProp test_prop_InsertModel_runner. *)
+
+Definition test_prop_DeleteModel   :=
+	@ForAllMaybe _ ∅ _ "t" (fun tt => spec_derived) (fun tt n => (fun n => spec_derived)) (fun tt n => shrink n) (fun tt n => show n) (
+	@ForAll _ (Tree · ∅) _ "k" (fun '(t, tt) => arbitrary) (fun '(t, tt) n => (fun n => arbitrary)) (fun '(t, tt) n => shrink n) (fun '(t, tt) n => show n) (
+	@Predicate (nat · (Tree · ∅)) Z
+	(fun '(k, (t, tt)) => (prop_DeleteModel t k, 0%Z)))).
+
+Definition test_prop_DeleteModel_runner := (targetLoop number_of_trials test_prop_DeleteModel (DynamicResettingSingletonPool.(mkPool) tt) DynamicResettingSingletonPool HillClimbingUtility).
+(*! QuickProp test_prop_DeleteModel_runner. *)
+
+Definition test_prop_UnionModel    :=
+	@ForAllMaybe _ ∅ _ "t" (fun tt => spec_derived) (fun tt n => (fun n => spec_derived)) (fun tt n => shrink n) (fun tt n => show n) (
+	@ForAllMaybe _ (Tree · ∅) _ "t'" (fun '(t, tt) => spec_derived) (fun '(t, tt) n => (fun n => spec_derived)) (fun '(t, tt) n => shrink n) (fun '(t, tt) n => show n) (
+	@Predicate (Tree · (Tree · ∅)) Z
+	(fun '(t', (t, tt)) => (prop_UnionModel t t', 0%Z)))).
+
+Definition test_prop_UnionModel_runner := (targetLoop number_of_trials test_prop_UnionModel (DynamicResettingSingletonPool.(mkPool) tt) DynamicResettingSingletonPool HillClimbingUtility).
+(*! QuickProp test_prop_UnionModel_runner. *)
+
+Definition test_prop_InsertInsert    :=
+	@ForAllMaybe _ ∅ _ "t" (fun tt => spec_derived) (fun tt n => (fun n => spec_derived)) (fun tt n => shrink n) (fun tt n => show n) (
+	@ForAll _ (Tree · ∅) _ "k" (fun '(t, tt) => arbitrary) (fun '(t, tt) n => (fun n => arbitrary)) (fun '(t, tt) n => shrink n) (fun '(t, tt) n => show n) (
+	@ForAll _ (nat · (Tree · ∅)) _ "k'" (fun '(k, (t, tt)) => arbitrary) (fun '(k, (t, tt)) n => (fun n => arbitrary)) (fun '(k, (t, tt)) n => shrink n) (fun '(k, (t, tt)) n => show n) (
+	@ForAll _ (nat · (nat · (Tree · ∅))) _ "v" (fun '(k', (k, (t, tt))) => arbitrary) (fun '(k', (k, (t, tt))) n => (fun n => arbitrary)) (fun '(k', (k, (t, tt))) n => shrink n) (fun '(k', (k, (t, tt))) n => show n) (
+	@ForAll _ (nat · (nat · (nat · (Tree · ∅)))) _ "v'" (fun '(v, (k', (k, (t, tt)))) => arbitrary) (fun '(v, (k', (k, (t, tt)))) n => (fun n => arbitrary)) (fun '(v, (k', (k, (t, tt)))) n => shrink n) (fun '(v, (k', (k, (t, tt)))) n => show n) (
+	@Predicate (nat · (nat · (nat · (nat · (Tree · ∅))))) Z
+	(fun '(v', (v, (k', (k, (t, tt))))) => (prop_InsertInsert t k k' v v', 0%Z))))))).
+
+Definition test_prop_InsertInsert_runner := (targetLoop number_of_trials test_prop_InsertInsert (DynamicResettingSingletonPool.(mkPool) tt) DynamicResettingSingletonPool HillClimbingUtility).
+(*! QuickProp test_prop_InsertInsert_runner. *)
+
+Definition test_prop_InsertDelete    :=
+	@ForAllMaybe _ ∅ _ "t" (fun tt => spec_derived) (fun tt n => (fun n => spec_derived)) (fun tt n => shrink n) (fun tt n => show n) (
+	@ForAll _ (Tree · ∅) _ "k" (fun '(t, tt) => arbitrary) (fun '(t, tt) n => (fun n => arbitrary)) (fun '(t, tt) n => shrink n) (fun '(t, tt) n => show n) (
+	@ForAll _ (nat · (Tree · ∅)) _ "k'" (fun '(k, (t, tt)) => arbitrary) (fun '(k, (t, tt)) n => (fun n => arbitrary)) (fun '(k, (t, tt)) n => shrink n) (fun '(k, (t, tt)) n => show n) (
+	@ForAll _ (nat · (nat · (Tree · ∅))) _ "v" (fun '(k', (k, (t, tt))) => arbitrary) (fun '(k', (k, (t, tt))) n => (fun n => arbitrary)) (fun '(k', (k, (t, tt))) n => shrink n) (fun '(k', (k, (t, tt))) n => show n) (
+	@Predicate (nat · (nat · (nat · (Tree · ∅)))) Z
+	(fun '(v, (k', (k, (t, tt)))) => (prop_InsertDelete t k k' v, 0%Z)))))).
+
+Definition test_prop_InsertDelete_runner := (targetLoop number_of_trials test_prop_InsertDelete (DynamicResettingSingletonPool.(mkPool) tt) DynamicResettingSingletonPool HillClimbingUtility).
+(*! QuickProp test_prop_InsertDelete_runner. *)
+
+Definition test_prop_InsertUnion   :=
+	@ForAllMaybe _ ∅ _ "t" (fun tt => spec_derived) (fun tt n => (fun n => spec_derived)) (fun tt n => shrink n) (fun tt n => show n) (
+	@ForAllMaybe _ (Tree · ∅) _ "t'" (fun '(t, tt) => spec_derived) (fun '(t, tt) n => (fun n => spec_derived)) (fun '(t, tt) n => shrink n) (fun '(t, tt) n => show n) (
+	@ForAll _ (Tree · (Tree · ∅)) _ "k" (fun '(t', (t, tt)) => arbitrary) (fun '(t', (t, tt)) n => (fun n => arbitrary)) (fun '(t', (t, tt)) n => shrink n) (fun '(t', (t, tt)) n => show n) (
+	@ForAll _ (nat · (Tree · (Tree · ∅))) _ "v" (fun '(k, (t', (t, tt))) => arbitrary) (fun '(k, (t', (t, tt))) n => (fun n => arbitrary)) (fun '(k, (t', (t, tt))) n => shrink n) (fun '(k, (t', (t, tt))) n => show n) (
+	@Predicate (nat · (nat · (Tree · (Tree · ∅)))) Z
+	(fun '(v, (k, (t', (t, tt)))) => (prop_InsertUnion t t' k v, 0%Z)))))).
+
+Definition test_prop_InsertUnion_runner := (targetLoop number_of_trials test_prop_InsertUnion (DynamicResettingSingletonPool.(mkPool) tt) DynamicResettingSingletonPool HillClimbingUtility).
+(*! QuickProp test_prop_InsertUnion_runner. *)
+
+Definition test_prop_DeleteInsert    :=
+	@ForAllMaybe _ ∅ _ "t" (fun tt => spec_derived) (fun tt n => (fun n => spec_derived)) (fun tt n => shrink n) (fun tt n => show n) (
+	@ForAll _ (Tree · ∅) _ "k" (fun '(t, tt) => arbitrary) (fun '(t, tt) n => (fun n => arbitrary)) (fun '(t, tt) n => shrink n) (fun '(t, tt) n => show n) (
+	@ForAll _ (nat · (Tree · ∅)) _ "k'" (fun '(k, (t, tt)) => arbitrary) (fun '(k, (t, tt)) n => (fun n => arbitrary)) (fun '(k, (t, tt)) n => shrink n) (fun '(k, (t, tt)) n => show n) (
+	@ForAll _ (nat · (nat · (Tree · ∅))) _ "v'" (fun '(k', (k, (t, tt))) => arbitrary) (fun '(k', (k, (t, tt))) n => (fun n => arbitrary)) (fun '(k', (k, (t, tt))) n => shrink n) (fun '(k', (k, (t, tt))) n => show n) (
+	@Predicate (nat · (nat · (nat · (Tree · ∅)))) Z
+	(fun '(v', (k', (k, (t, tt)))) => (prop_DeleteInsert t k k' v', 0%Z)))))).
+
+Definition test_prop_DeleteInsert_runner := (targetLoop number_of_trials test_prop_DeleteInsert (DynamicResettingSingletonPool.(mkPool) tt) DynamicResettingSingletonPool HillClimbingUtility).
+(*! QuickProp test_prop_DeleteInsert_runner. *)
+
+Definition test_prop_DeleteDelete    :=
+	@ForAllMaybe _ ∅ _ "t" (fun tt => spec_derived) (fun tt n => (fun n => spec_derived)) (fun tt n => shrink n) (fun tt n => show n) (
+	@ForAll _ (Tree · ∅) _ "k" (fun '(t, tt) => arbitrary) (fun '(t, tt) n => (fun n => arbitrary)) (fun '(t, tt) n => shrink n) (fun '(t, tt) n => show n) (
+	@ForAll _ (nat · (Tree · ∅)) _ "k'" (fun '(k, (t, tt)) => arbitrary) (fun '(k, (t, tt)) n => (fun n => arbitrary)) (fun '(k, (t, tt)) n => shrink n) (fun '(k, (t, tt)) n => show n) (
+	@Predicate (nat · (nat · (Tree · ∅))) Z
+	(fun '(k', (k, (t, tt))) => ((prop_DeleteDelete t k k', 0%Z)))))).
+
+Definition test_prop_DeleteDelete_runner := (targetLoop number_of_trials test_prop_DeleteDelete (DynamicResettingSingletonPool.(mkPool) tt) DynamicResettingSingletonPool HillClimbingUtility).
+(*! QuickProp test_prop_DeleteDelete_runner. *)
+
+Definition test_prop_DeleteUnion   :=
+	@ForAllMaybe _ ∅ _ "t" (fun tt => spec_derived) (fun tt n => (fun n => spec_derived)) (fun tt n => shrink n) (fun tt n => show n) (
+	@ForAllMaybe _ (Tree · ∅) _ "t'" (fun '(t, tt) => spec_derived) (fun '(t, tt) n => (fun n => spec_derived)) (fun '(t, tt) n => shrink n) (fun '(t, tt) n => show n) (
+	@ForAll _ (Tree · (Tree · ∅)) _ "k" (fun '(t', (t, tt)) => arbitrary) (fun '(t', (t, tt)) n => (fun n => arbitrary)) (fun '(t', (t, tt)) n => shrink n) (fun '(t', (t, tt)) n => show n) (
+	@Predicate (nat · (Tree · (Tree · ∅))) Z
+	(fun '(k, (t', (t, tt))) => (prop_DeleteUnion t t' k, 0%Z))))).
+
+Definition test_prop_DeleteUnion_runner := (targetLoop number_of_trials test_prop_DeleteUnion (DynamicResettingSingletonPool.(mkPool) tt) DynamicResettingSingletonPool HillClimbingUtility).
+(*! QuickProp test_prop_DeleteUnion_runner. *)
+
+Definition test_prop_UnionDeleteInsert   :=
+	@ForAllMaybe _ ∅ _ "t " (fun tt => spec_derived) (fun tt n => (fun n => spec_derived)) (fun tt n => shrink n) (fun tt n => show n) (
+	@ForAllMaybe _ (Tree · ∅) _ "t'" (fun '(t , tt) => spec_derived) (fun '(t , tt) n => (fun n => spec_derived)) (fun '(t , tt) n => shrink n) (fun '(t , tt) n => show n) (
+	@ForAll _ (Tree · (Tree · ∅)) _ "k" (fun '(t', (t , tt)) => arbitrary) (fun '(t', (t , tt)) n => (fun n => arbitrary)) (fun '(t', (t , tt)) n => shrink n) (fun '(t', (t , tt)) n => show n) (
+	@ForAll _ (nat · (Tree · (Tree · ∅))) _ "v" (fun '(k, (t', (t , tt))) => arbitrary) (fun '(k, (t', (t , tt))) n => (fun n => arbitrary)) (fun '(k, (t', (t , tt))) n => shrink n) (fun '(k, (t', (t , tt))) n => show n) (
+	@Predicate (nat · (nat · (Tree · (Tree · ∅)))) Z
+	(fun '(v, (k, (t', (t, tt)))) => ((prop_UnionDeleteInsert t t' k v, 0%Z))))))).
+
+Definition test_prop_UnionDeleteInsert_runner := (targetLoop number_of_trials test_prop_UnionDeleteInsert (DynamicResettingSingletonPool.(mkPool) tt) DynamicResettingSingletonPool HillClimbingUtility).
+(*! QuickProp test_prop_UnionDeleteInsert_runner. *)
+
+Definition test_prop_UnionUnionIdem    :=
+	@ForAllMaybe _ ∅ _ "t" (fun tt => spec_derived) (fun tt n => (fun n => spec_derived)) (fun tt n => shrink n) (fun tt n => show n) (
+	@Predicate (Tree · ∅) Z
+	(fun '(t, tt) => (prop_UnionUnionIdem t, 0%Z))).
+
+Definition test_prop_UnionUnionIdem_runner := (targetLoop number_of_trials test_prop_UnionUnionIdem (DynamicResettingSingletonPool.(mkPool) tt) DynamicResettingSingletonPool HillClimbingUtility).
+(*! QuickProp test_prop_UnionUnionIdem_runner. *)
+
+Definition test_prop_UnionUnionAssoc   :=
+	@ForAllMaybe _ ∅ _ "t1" (fun tt => spec_derived) (fun tt n => (fun n => spec_derived)) (fun tt n => shrink n) (fun tt n => show n) (
+	@ForAllMaybe _ (Tree · ∅) _ "t2" (fun '(t1, tt) => spec_derived) (fun '(t1, tt) n => (fun n => spec_derived)) (fun '(t1, tt) n => shrink n) (fun '(t1, tt) n => show n) (
+	@ForAllMaybe _ (Tree · (Tree · ∅)) _ "t3" (fun '(t2, (t1, tt)) => spec_derived) (fun '(t2, (t1, tt)) n => (fun n => spec_derived)) (fun '(t2, (t1, tt)) n => shrink n) (fun '(t2, (t1, tt)) n => show n) (
+	@Predicate (Tree · (Tree · (Tree · ∅))) Z
+	(fun '(t3, (t2, (t1, tt))) => (prop_UnionUnionAssoc t1 t2 t3, 0%Z))))).
+
+Definition test_prop_UnionUnionAssoc_runner := (targetLoop number_of_trials test_prop_UnionUnionAssoc (DynamicResettingSingletonPool.(mkPool) tt) DynamicResettingSingletonPool HillClimbingUtility).
+(*! QuickProp test_prop_UnionUnionAssoc_runner. *)
