workloads/Coq/RBTProplang/Runners/TypeBasedGenerator_test_runner.v
@@ -1,0 +1,33 @@
+From RBTProplang Require Import TypeBasedGenerator.
+From QuickChick Require Import QuickChick.
+Set Warnings "-extraction-opaque-accessed,-extraction".
+Axiom num_tests : nat. Extract Constant num_tests => "max_int".
+Definition qctest_test_prop_InsertValid_runner := (fun _ : unit => print_extracted_coq_string ("[|{" ++ show (withTime(fun tt => (sample1 test_prop_InsertValid_runner))) ++ "}|]")).
+Definition qctest_test_prop_DeleteValid_runner := (fun _ : unit => print_extracted_coq_string ("[|{" ++ show (withTime(fun tt => (sample1 test_prop_DeleteValid_runner))) ++ "}|]")).
+Definition qctest_test_prop_InsertPost_runner := (fun _ : unit => print_extracted_coq_string ("[|{" ++ show (withTime(fun tt => (sample1 test_prop_InsertPost_runner))) ++ "}|]")).
+Definition qctest_test_prop_DeletePost_runner := (fun _ : unit => print_extracted_coq_string ("[|{" ++ show (withTime(fun tt => (sample1 test_prop_DeletePost_runner))) ++ "}|]")).
+Definition qctest_test_prop_InsertModel_runner := (fun _ : unit => print_extracted_coq_string ("[|{" ++ show (withTime(fun tt => (sample1 test_prop_InsertModel_runner))) ++ "}|]")).
+Definition qctest_test_prop_DeleteModel_runner := (fun _ : unit => print_extracted_coq_string ("[|{" ++ show (withTime(fun tt => (sample1 test_prop_DeleteModel_runner))) ++ "}|]")).
+Definition qctest_test_prop_InsertInsert_runner := (fun _ : unit => print_extracted_coq_string ("[|{" ++ show (withTime(fun tt => (sample1 test_prop_InsertInsert_runner))) ++ "}|]")).
+Definition qctest_test_prop_InsertDelete_runner := (fun _ : unit => print_extracted_coq_string ("[|{" ++ show (withTime(fun tt => (sample1 test_prop_InsertDelete_runner))) ++ "}|]")).
+Definition qctest_test_prop_DeleteInsert_runner := (fun _ : unit => print_extracted_coq_string ("[|{" ++ show (withTime(fun tt => (sample1 test_prop_DeleteInsert_runner))) ++ "}|]")).
+Definition qctest_test_prop_DeleteDelete_runner := (fun _ : unit => print_extracted_coq_string ("[|{" ++ show (withTime(fun tt => (sample1 test_prop_DeleteDelete_runner))) ++ "}|]")).
+
+
+Parameter OCamlString : Type.
+Extract Constant OCamlString => "string".
+Axiom qctest_map : OCamlString -> unit.
+Extract Constant qctest_map => "
+fun test_name ->
+  let test_map = [
+    (""test_prop_InsertValid_runner"", qctest_test_prop_InsertValid_runner); (""test_prop_DeleteValid_runner"", qctest_test_prop_DeleteValid_runner); (""test_prop_InsertPost_runner"", qctest_test_prop_InsertPost_runner); (""test_prop_DeletePost_runner"", qctest_test_prop_DeletePost_runner); (""test_prop_InsertModel_runner"", qctest_test_prop_InsertModel_runner); (""test_prop_DeleteModel_runner"", qctest_test_prop_DeleteModel_runner); (""test_prop_InsertInsert_runner"", qctest_test_prop_InsertInsert_runner); (""test_prop_InsertDelete_runner"", qctest_test_prop_InsertDelete_runner); (""test_prop_DeleteInsert_runner"", qctest_test_prop_DeleteInsert_runner); (""test_prop_DeleteDelete_runner"", qctest_test_prop_DeleteDelete_runner)
+  ] in
+  let test = List.assoc test_name test_map in
+  test ()
+
+let () =
+Sys.argv.(1) |> qctest_map
+
+".
+
+Extraction "TypeBasedGenerator_test_runner.ml" qctest_test_prop_InsertValid_runner qctest_test_prop_DeleteValid_runner qctest_test_prop_InsertPost_runner qctest_test_prop_DeletePost_runner qctest_test_prop_InsertModel_runner qctest_test_prop_DeleteModel_runner qctest_test_prop_InsertInsert_runner qctest_test_prop_InsertDelete_runner qctest_test_prop_DeleteInsert_runner qctest_test_prop_DeleteDelete_runner qctest_map.
