workloads/Coq/RBTProplang/Src/Impl.v
@@ -1,0 +1,283 @@
+
+Require Import ZArith.
+From QuickChick Require Import QuickChick.
+From ExtLib Require Import Monad.
+From ExtLib.Data.Monads Require Import OptionMonad.
+Import QcNotation.
+Import MonadNotation.
+From Coq Require Import List.
+Import ListNotations.
+
+
+Local Open Scope Z_scope.
+
+Notation "A <?? B" := (Z_lt_le_dec A B) (at level 70, no associativity).
+
+
+Inductive Color := R | B.
+Derive (Arbitrary, Show) for Color.
+
+
+Inductive Tree :=
+    | E : Tree
+    | T : Color -> Tree -> Z -> Z -> Tree -> Tree.
+
+Derive (Show) for Tree.
+
+Axiom fuel : nat. Extract Constant fuel => "100000".
+
+(* ---------- *)
+
+(* -- Used for insert and delete. *)
+
+Definition blacken (t: Tree) : Tree :=
+    match t with
+    | E => E
+    | (T _ a x vx b) => T B a x vx b
+    end.
+
+
+Definition redden (t: Tree) : option Tree :=
+    match t with
+    | T B a x vx b => Some(T R a x vx b)
+    | _ => None
+    end.
+
+Definition balance (col: Color) (tl: Tree) (key: Z) (val: Z) (tr: Tree) : Tree :=
+    match col, tl, key, val, tr with
+    (*! *)
+    | B, (T R (T R a x vx b) y vy c), z, vz, d => T R (T B a x vx b) y vy (T B c z vz d)
+(*!! swap_cd *)
+(*! 
+    | B, (T R (T R a x vx b) y vy c), z, vz, d => T R (T B a x vx b) y vy (T B d z vz c) 
+*)
+    | B, (T R a x vx (T R b y vy c)), z, vz, d => T R (T B a x vx b) y vy (T B c z vz d)
+(*! *)
+    | B, a, x, vx, (T R (T R b y vy c) z vz d) => T R (T B a x vx b) y vy (T B c z vz d)
+(*!! swap_bc *)
+(*! 
+    | B, a, x, vx, (T R (T R b y vy c) z vz d) => T R (T B a x vx c) y vy (T B b z vz d) 
+*)
+    | B, a, x, vx, (T R b y vy (T R c z vz d)) => T R (T B a x vx b) y vy (T B c z vz d)
+    | rb, a, x, vx, b => T rb a x vx b
+    end.
+
+(* ----------
+ *)
+Set Warnings "-non-recursive, -fixpoints".
+Fixpoint insert (key: Z) (val: Z) (t: Tree) : Tree :=
+    let fix ins (x: Z) (vx: Z) (s: Tree) : Tree :=
+    match x, vx, s with
+    | x, vx, E => 
+    (*! *)
+    T R E x vx E
+    (*!! miscolor_insert *)
+    (*! 
+    T B E x vx E 
+    *)
+    | x, vx, (T rb a y vy b) =>
+    (*! *)
+    if x <?? y then balance rb (ins x vx a) y vy b
+    else if y <?? x then balance rb a y vy (ins x vx b)
+    else T rb a y vx b
+    (*!! insert_1 *)
+    (*!
+    T R E x vx E
+    *)
+    (*!! insert_2 *)
+    (*!
+    if x <?? y then balance rb (ins x vx a) y vy b
+    else T rb a y vx b
+    *)
+    (*!! insert_3 *)
+    (*!
+    if x <?? y then balance rb (ins x vx a) y vy b
+    else if y <?? x then balance rb a y vy (ins x vx b)
+    else T rb a y vy b
+    *)
+    (*!! no_balance_insert_1 *)
+    (*!
+    if x <?? y then T rb (ins x vx a) y vy b
+    else if y <?? x then balance rb a y vy (ins x vx b)
+    else T rb a y vx b
+    *)
+    (*!! no_balance_insert_2 *)
+    (*!
+    if x <?? y then balance rb (ins x vx a) y vy b
+    else if y <?? x then T rb a y vy (insert x vx b)
+    else T rb a y vx b
+    *)
+    end
+    in blacken (ins key val t).
+
+Set Warnings "+non-recursive, +fixpoints".
+
+(* -- Based on https://www.cs.kent.ac.uk/people/staff/smk/redblack/Untyped.hs *)
+
+Definition balLeft (tl: Tree) (k: Z) (v: Z) (tr: Tree) : option Tree :=
+    match tl, k, v, tr with
+    | (T R a x vx b), y, vy, c => Some (T R (T B a x vx b) y vy c)
+    | bl, x, vx, (T B a y vy b) => Some (balance B bl x vx (T R a y vy b))
+    | bl, x, vx, (T R (T B a y vy b) z vz c) =>
+  (*! *)
+    c' <- (redden c) ;;
+    Some (T R (T B bl x vx a) y vy (balance B b z vz c'))
+  (*!! miscolor_balLeft *) 
+  (*! 
+  Some (T R (T B bl x vx a) y vy (balance B b z vz c) )
+  *)
+    | _, _, _, _ => None
+    end.
+
+
+Definition balRight (tl: Tree) (k: Z) (v: Z) (tr: Tree) : option Tree :=
+    match tl, k, v, tr with
+    | a, x, vx, (T R b y vy c) => Some(T R a x vx (T B b y vy c))
+    | (T B a x vx b), y, vy, bl => Some(balance B (T R a x vx b) y vy bl)
+    | (T R a x vx (T B b y vy c)), z, vz, bl =>
+    (*! *)
+        a' <- redden a ;;
+        Some (T R (balance B a' x vx b) y vy (T B c z vz bl))
+    (*!! miscolor_balRight *) 
+    (*! 
+        Some (T R (balance B a x vx b) y vy (T B c z vz bl) )
+    *)
+    | _, _, _, _ => None
+    end.
+
+Fixpoint _join (t1: Tree) (t2: Tree) (f: nat) : option Tree :=
+    match f with
+    | O => None
+    | S f' =>
+        match t1, t2 with
+        | E, a => Some a
+        | a, E => Some a
+        | (T R a x vx b), (T R c y vy d) =>
+            match _join b c f' with
+            | None => None
+            | Some(T R b' z vz c') => 
+            (*! *)
+                Some (T R (T R a x vx b') z vz (T R c' y vy d))
+            (*!! miscolor_join_1 *)
+            (*! Some(T R (T B a x vx b') z vz (T B c' y vy d)) *)
+            | Some(bc) => Some(T R a x vx (T R bc y vy d))
+            end
+        | (T B a x vx b), (T B c y vy d) =>
+            match _join b c f' with
+            | None => None
+            | Some(T R b' z vz c') => 
+            (*! *)
+            Some(T R (T B a x vx b') z vz (T B c' y vy d))
+            (*!! miscolor_join_2 *)
+            (*! 
+            Some(T R (T R a x vx b') z vz (T R c' y vy d))
+            *)
+            | Some(bc) => 
+                balLeft a x vx (T B bc y vy d)
+            end
+        | a, (T R b x vx c) => 
+            match _join a b f' with
+            | None => None
+            | Some t' =>
+                Some (T R t' x vx c)
+            end
+        | (T R a x vx b), c => 
+            t' <- _join b c f' ;;
+            Some (T R a x vx t')
+        end 
+    end.
+
+Definition join (t1: Tree) (t2: Tree) : option Tree :=
+    _join t1 t2 fuel.
+(* ---------- *)
+
+
+Fixpoint del (x: Z) (s: Tree) (f: nat) : option Tree :=
+    match f with
+    | O => None
+    | S f' =>
+        match s with
+        | E => Some E
+        | (T _ a y vy b) =>
+            (*! *)
+            if x <?? y then 
+                t' <- delLeft x a y vy b f' ;;
+                Some t'
+            else if y <?? x then 
+                t' <- delRight x a y vy b f' ;;
+                Some t'
+            else 
+                t' <- join a b ;;
+                Some t'
+            (*!! delete_4 *)
+            (*!
+            let _tmp := delLeft in
+            let _tmp := delRight in
+            if x <?? y then del x a f'
+            else if y <?? x then del x b f'
+            else join a b 
+            *)
+            (*!! delete_5 *)
+            (*!
+            if y <?? x then delLeft x a y vy b f'
+            else if x <?? y then delRight x a y vy b f'
+            else join a b
+            *)
+        end
+    end
+with delLeft (x: Z) (dl: Tree) (dy: Z) (dvy: Z) (dr: Tree) (f: nat): option Tree :=
+    match f with
+    | O => None
+    | S f' =>
+        match dl, dy, dvy, dr with
+        | (T B al ax avx ar), y, vy, b => 
+            t' <- (del x (T B al ax avx ar) f') ;;
+            t'' <- balLeft t' y vy b ;;
+            Some t''
+        | a, y, vy, b => 
+            t' <- del x a f' ;;
+            Some (T R t' y vy b)
+        end
+    end
+with delRight (x: Z) (dl: Tree) (dy: Z) (dvy: Z) (dr: Tree) (f: nat): option Tree :=
+    match f with
+    | O => None
+    | S f' =>
+        match dl, dy, dvy, dr with
+        | a, y, vy, (T B bl bx bvx br) => 
+            t' <- (del x (T B bl bx bvx br) f') ;;
+            t'' <- balRight a y vy t' ;;
+            Some t''
+        | a, y, vy, b => 
+            t' <- del x b f' ;;
+            Some (T R a y vy t')
+        end
+    end.
+
+Definition delete (x: Z) (t: Tree) : option Tree :=
+    (*! *)
+    t' <- del x t fuel ;;
+    Some (blacken t')
+    (*!! miscolor_delete *)
+    (*!
+    del x t fuel
+    *)
+    .
+
+
+
+Fixpoint find (x: Z) (t: Tree) : option Z :=
+    match t with
+    | E => None
+    | (T _ l y vy r) =>
+        if x <?? y then find x l
+        else if y <?? x then find x r
+        else (Some vy)
+    end.
+
+
+Fixpoint size (t: Tree) : nat :=
+  match t with
+  | E => 0
+  | T c l k v r => 1 + size l + size r
+  end.
