workloads/Coq/RBTProplang/Strategies/BespokeGenerator.v
@@ -1,0 +1,181 @@
+
+
+
+Require Import ZArith.
+From QuickChick Require Import QuickChick.
+From ExtLib Require Import Monad.
+From ExtLib.Data.Monads Require Import OptionMonad.
+Import QcNotation.
+Import MonadNotation.
+From Coq Require Import List.
+Import ListNotations.
+
+From RBTProplang Require Import Impl Spec PropLang.
+
+Local Open Scope prop_scope.
+Open Scope Z_scope.
+
+Derive (Shrink) for Tree.
+Definition genZ := choose (-20, 20).
+
+Fixpoint gen_kvs (s : nat) : G (list (Z * Z)) :=
+  match s with
+  | O => ret []
+  | S s' => k <- genZ;;
+           v <- arbitrary;;
+           kvs <- gen_kvs s';;
+           ret ((k, v) :: kvs)
+  end.
+
+Definition blacken_ (t: Tree) : Tree :=
+    match t with
+    | E => E
+    | (T _ a x vx b) => T B a x vx b
+    end.
+
+Definition balance_ (col: Color) (tl: Tree) (key: Z) (val: Z) (tr: Tree) : Tree :=
+    match col, tl, key, val, tr with
+    | B, (T R (T R a x vx b) y vy c), z, vz, d => T R (T B a x vx b) y vy (T B c z vz d)
+    | B, (T R a x vx (T R b y vy c)), z, vz, d => T R (T B a x vx b) y vy (T B c z vz d)
+    | B, a, x, vx, (T R (T R b y vy c) z vz d) => T R (T B a x vx b) y vy (T B c z vz d)
+    | B, a, x, vx, (T R b y vy (T R c z vz d)) => T R (T B a x vx b) y vy (T B c z vz d)
+    | rb, a, x, vx, b => T rb a x vx b
+    end.
+
+
+Fixpoint insert_ (key: Z) (val: Z) (t: Tree) : Tree :=
+    let fix ins (x: Z) (vx: Z) (s: Tree) : Tree :=
+    match x, vx, s with
+    | x, vx, E => 
+    T R E x vx E
+    | x, vx, (T rb a y vy b) =>
+    if x <?? y then balance_ rb (ins x vx a) y vy b
+    else if y <?? x then balance_ rb a y vy (ins x vx b)
+    else T rb a y vx b
+    end
+    in blacken_ (ins key val t).
+
+Definition gen_tree (s : nat) : G Tree :=
+    sz <- choose(1, s)%nat;;
+    kvs <- gen_kvs sz;;
+    ret (fold_right (fun '(k, v) t => insert_ k v t) E kvs).
+
+Definition bespoke :=
+    gen_tree 20.
+    
+#[local] Instance dec_eq_tree : Dec_Eq Tree.
+Proof. dec_eq. Defined.
+    
+
+Axiom number_of_trials : nat.
+Extract Constant number_of_trials => "20000".
+
+(* --------------------- Tests --------------------- *)
+
+Definition test_prop_InsertValid   :=
+	@ForAll _ ∅ _ "t" (fun tt => bespoke) (fun tt n => (fun n => bespoke)) (fun tt n => shrink n) (fun tt n => show n) (
+	@ForAll _ (Tree · ∅) _ "k" (fun '(t, tt) => genZ) (fun '(t, tt) n => (fun n => genZ)) (fun '(t, tt) n => shrink n) (fun '(t, tt) n => show n) (
+	@ForAll _ (Z · (Tree · ∅)) _ "v" (fun '(k, (t, tt)) => arbitrary) (fun '(k, (t, tt)) n => (fun n => arbitrary)) (fun '(k, (t, tt)) n => shrink n) (fun '(k, (t, tt)) n => show n) (
+	@Predicate (Z · (Z · (Tree · ∅))) Z
+	(fun '(v, (k, (t, tt))) => (prop_InsertValid t k v, 0))))).
+
+Definition test_prop_InsertValid_runner := (targetLoop number_of_trials test_prop_InsertValid (DynamicResettingSingletonPool.(mkPool) tt) DynamicResettingSingletonPool HillClimbingUtility).
+
+(*! QuickProp test_prop_InsertValid_runner. *)
+
+Definition test_prop_DeleteValid   :=
+	@ForAll _ ∅ _ "t" (fun tt => bespoke) (fun tt n => (fun n => bespoke)) (fun tt n => shrink n) (fun tt n => show n) (
+	@ForAll _ (Tree · ∅) _ "k" (fun '(t, tt) => genZ) (fun '(t, tt) n => (fun n => genZ)) (fun '(t, tt) n => shrink n) (fun '(t, tt) n => show n) (
+	@Predicate (Z · (Tree · ∅)) Z
+	(fun '(k, (t, tt)) => (prop_DeleteValid t k, 0)))).
+
+Definition test_prop_DeleteValid_runner := (targetLoop number_of_trials test_prop_DeleteValid (DynamicResettingSingletonPool.(mkPool) tt) DynamicResettingSingletonPool HillClimbingUtility).
+
+(*! QuickProp test_prop_DeleteValid_runner. *)
+
+Definition test_prop_InsertPost    :=
+	@ForAll _ ∅ _ "t" (fun tt => bespoke) (fun tt n => (fun n => bespoke)) (fun tt n => shrink n) (fun tt n => show n) (
+	@ForAll _ (Tree · ∅) _ "k" (fun '(t, tt) => genZ) (fun '(t, tt) n => (fun n => genZ)) (fun '(t, tt) n => shrink n) (fun '(t, tt) n => show n) (
+	@ForAll _ (Z · (Tree · ∅)) _ "k'" (fun '(k, (t, tt)) => genZ) (fun '(k, (t, tt)) n => (fun n => genZ)) (fun '(k, (t, tt)) n => shrink n) (fun '(k, (t, tt)) n => show n) (
+	@ForAll _ (Z · (Z · (Tree · ∅))) _ "v" (fun '(k', (k, (t, tt))) => arbitrary) (fun '(k', (k, (t, tt))) n => (fun n => arbitrary)) (fun '(k', (k, (t, tt))) n => shrink n) (fun '(k', (k, (t, tt))) n => show n) (
+	@Predicate (Z · (Z · (Z · (Tree · ∅)))) Z
+	(fun '(v, (k', (k, (t, tt)))) => (prop_InsertPost t k k' v, 0%Z)))))).
+
+Definition test_prop_InsertPost_runner := (targetLoop number_of_trials test_prop_InsertPost (DynamicResettingSingletonPool.(mkPool) tt) DynamicResettingSingletonPool HillClimbingUtility).
+(*! QuickProp test_prop_InsertPost_runner. *)
+
+Definition test_prop_DeletePost    :=
+	@ForAll _ ∅ _ "t" (fun tt => bespoke) (fun tt n => (fun n => bespoke)) (fun tt n => shrink n) (fun tt n => show n) (
+	@ForAll _ (Tree · ∅) _ "k" (fun '(t, tt) => genZ) (fun '(t, tt) n => (fun n => genZ)) (fun '(t, tt) n => shrink n) (fun '(t, tt) n => show n) (
+	@ForAll _ (Z · (Tree · ∅)) _ "k'" (fun '(k, (t, tt)) => genZ) (fun '(k, (t, tt)) n => (fun n => genZ)) (fun '(k, (t, tt)) n => shrink n) (fun '(k, (t, tt)) n => show n) (
+	@Predicate (Z · (Z · (Tree · ∅))) Z
+	(fun '(k', (k, (t, tt))) => (prop_DeletePost t k k', 0%Z))))).
+
+Definition test_prop_DeletePost_runner := (targetLoop number_of_trials test_prop_DeletePost (DynamicResettingSingletonPool.(mkPool) tt) DynamicResettingSingletonPool HillClimbingUtility).
+(*! QuickProp test_prop_DeletePost_runner. *)
+
+Definition test_prop_InsertModel    :=
+	@ForAll _ ∅ _ "t" (fun tt => bespoke) (fun tt n => (fun n => bespoke)) (fun tt n => shrink n) (fun tt n => show n) (
+	@ForAll _ (Tree · ∅) _ "k" (fun '(t, tt) => genZ) (fun '(t, tt) n => (fun n => genZ)) (fun '(t, tt) n => shrink n) (fun '(t, tt) n => show n) (
+	@ForAll _ (Z · (Tree · ∅)) _ "v'" (fun '(v, (t, tt)) => arbitrary) (fun '(v, (t, tt)) n => (fun n => arbitrary)) (fun '(v, (t, tt)) n => shrink n) (fun '(v, (t, tt)) n => show n) (
+	@Predicate (Z · (Z · (Tree · ∅))) Z
+	(fun '(v, (k, (t, tt))) => (prop_InsertModel t k v, 0%Z))))).
+
+    
+Definition test_prop_InsertModel_runner := (targetLoop number_of_trials test_prop_InsertModel (DynamicResettingSingletonPool.(mkPool) tt) DynamicResettingSingletonPool HillClimbingUtility).
+(*! QuickProp test_prop_InsertModel_runner. *)
+
+Definition test_prop_DeleteModel    :=
+	@ForAll _ ∅ _ "t" (fun tt => bespoke) (fun tt n => (fun n => bespoke)) (fun tt n => shrink n) (fun tt n => show n) (
+	@ForAll _ (Tree · ∅) _ "k" (fun '(t, tt) => genZ) (fun '(t, tt) n => (fun n => genZ)) (fun '(t, tt) n => shrink n) (fun '(t, tt) n => show n) (
+	@Predicate (Z · (Tree · ∅)) Z
+	(fun '(k, (t, tt)) => (prop_DeleteModel t k, 0%Z)))).
+
+    
+Definition test_prop_DeleteModel_runner := (targetLoop number_of_trials test_prop_DeleteModel (DynamicResettingSingletonPool.(mkPool) tt) DynamicResettingSingletonPool HillClimbingUtility).
+(*! QuickProp test_prop_DeleteModel_runner. *)
+
+Definition test_prop_InsertInsert    :=
+	@ForAll _ ∅ _ "t" (fun tt => bespoke) (fun tt n => (fun n => bespoke)) (fun tt n => shrink n) (fun tt n => show n) (
+	@ForAll _ (Tree · ∅) _ "k" (fun '(t, tt) => genZ) (fun '(t, tt) n => (fun n => genZ)) (fun '(t, tt) n => shrink n) (fun '(t, tt) n => show n) (
+	@ForAll _ (Z · (Tree · ∅)) _ "k'" (fun '(k, (t, tt)) => genZ) (fun '(k, (t, tt)) n => (fun n => genZ)) (fun '(k, (t, tt)) n => shrink n) (fun '(k, (t, tt)) n => show n) (
+	@ForAll _ (Z · (Z · (Tree · ∅))) _ "v" (fun '(k', (k, (t, tt))) => arbitrary) (fun '(k', (k, (t, tt))) n => (fun n => arbitrary)) (fun '(k', (k, (t, tt))) n => shrink n) (fun '(k', (k, (t, tt))) n => show n) (
+	@ForAll _ (Z · (Z · (Z · (Tree · ∅)))) _ "v'" (fun '(v, (k', (k, (t, tt)))) => arbitrary) (fun '(v, (k', (k, (t, tt)))) n => (fun n => arbitrary)) (fun '(v, (k', (k, (t, tt)))) n => shrink n) (fun '(v, (k', (k, (t, tt)))) n => show n) (
+	@Predicate (Z · (Z · (Z · (Z · (Tree · ∅))))) Z
+	(fun '(v', (v, (k', (k, (t, tt))))) => (prop_InsertInsert t k k' v v', 0%Z))))))).
+
+Definition test_prop_InsertInsert_runner := (targetLoop number_of_trials test_prop_InsertInsert (DynamicResettingSingletonPool.(mkPool) tt) DynamicResettingSingletonPool HillClimbingUtility).
+(*! QuickProp test_prop_InsertInsert_runner. *)
+
+Definition test_prop_InsertDelete    :=
+	@ForAll _ ∅ _ "t" (fun tt => bespoke) (fun tt n => (fun n => bespoke)) (fun tt n => shrink n) (fun tt n => show n) (
+	@ForAll _ (Tree · ∅) _ "k" (fun '(t, tt) => genZ) (fun '(t, tt) n => (fun n => genZ)) (fun '(t, tt) n => shrink n) (fun '(t, tt) n => show n) (
+	@ForAll _ (Z · (Tree · ∅)) _ "k'" (fun '(k, (t, tt)) => genZ) (fun '(k, (t, tt)) n => (fun n => genZ)) (fun '(k, (t, tt)) n => shrink n) (fun '(k, (t, tt)) n => show n) (
+	@ForAll _ (Z · (Z · (Tree · ∅))) _ "v" (fun '(k', (k, (t, tt))) => arbitrary) (fun '(k', (k, (t, tt))) n => (fun n => arbitrary)) (fun '(k', (k, (t, tt))) n => shrink n) (fun '(k', (k, (t, tt))) n => show n) (
+	@Predicate (Z · (Z · (Z · (Tree · ∅)))) Z
+	(fun '(v, (k', (k, (t, tt)))) => (prop_InsertDelete t k k' v, 0%Z)))))).
+
+Definition test_prop_InsertDelete_runner := (targetLoop number_of_trials test_prop_InsertDelete (DynamicResettingSingletonPool.(mkPool) tt) DynamicResettingSingletonPool HillClimbingUtility).
+(*! QuickProp test_prop_InsertDelete_runner. *)
+
+
+Definition test_prop_DeleteInsert    :=
+	@ForAll _ ∅ _ "t" (fun tt => bespoke) (fun tt n => (fun n => bespoke)) (fun tt n => shrink n) (fun tt n => show n) (
+	@ForAll _ (Tree · ∅) _ "k" (fun '(t, tt) => genZ) (fun '(t, tt) n => (fun n => genZ)) (fun '(t, tt) n => shrink n) (fun '(t, tt) n => show n) (
+	@ForAll _ (Z · (Tree · ∅)) _ "k'" (fun '(k, (t, tt)) => genZ) (fun '(k, (t, tt)) n => (fun n => genZ)) (fun '(k, (t, tt)) n => shrink n) (fun '(k, (t, tt)) n => show n) (
+	@ForAll _ (Z · (Z · (Tree · ∅))) _ "v'" (fun '(k', (k, (t, tt))) => arbitrary) (fun '(k', (k, (t, tt))) n => (fun n => arbitrary)) (fun '(k', (k, (t, tt))) n => shrink n) (fun '(k', (k, (t, tt))) n => show n) (
+	@Predicate (Z · (Z · (Z · (Tree · ∅)))) Z
+	(fun '(v', (k', (k, (t, tt)))) => (prop_DeleteInsert t k k' v', 0%Z)))))).
+
+Definition test_prop_DeleteInsert_runner := (targetLoop number_of_trials test_prop_DeleteInsert (DynamicResettingSingletonPool.(mkPool) tt) DynamicResettingSingletonPool HillClimbingUtility).
+(*! QuickProp test_prop_DeleteInsert_runner. *)
+
+Definition test_prop_DeleteDelete    :=
+	@ForAll _ ∅ _ "t" (fun tt => bespoke) (fun tt n => (fun n => bespoke)) (fun tt n => shrink n) (fun tt n => show n) (
+	@ForAll _ (Tree · ∅) _ "k" (fun '(t, tt) => genZ) (fun '(t, tt) n => (fun n => genZ)) (fun '(t, tt) n => shrink n) (fun '(t, tt) n => show n) (
+	@ForAll _ (Z · (Tree · ∅)) _ "k'" (fun '(k, (t, tt)) => genZ) (fun '(k, (t, tt)) n => (fun n => genZ)) (fun '(k, (t, tt)) n => shrink n) (fun '(k, (t, tt)) n => show n) (
+	@Predicate (Z · (Z · (Tree · ∅))) Z
+	(fun '(k', (k, (t, tt))) => ((prop_DeleteDelete t k k', 0%Z)))))).
+
+Definition test_prop_DeleteDelete_runner := (targetLoop number_of_trials test_prop_DeleteDelete (DynamicResettingSingletonPool.(mkPool) tt) DynamicResettingSingletonPool HillClimbingUtility).
+(*! QuickProp test_prop_DeleteDelete_runner. *)
