workloads/Coq/RBTProplang/Strategies/TypeBasedGenerator.v
@@ -1,0 +1,137 @@
+
+
+
+Require Import ZArith.
+From QuickChick Require Import QuickChick.
+From ExtLib Require Import Monad.
+From ExtLib.Data.Monads Require Import OptionMonad.
+Import QcNotation.
+Import MonadNotation.
+From Coq Require Import List.
+Import ListNotations.
+
+
+From RBTProplang Require Import Impl Spec PropLang.
+Local Open Scope prop_scope.
+
+(* --------------------- Generator --------------------- *)
+
+Derive (Arbitrary, Shrink) for Tree.
+
+#[local] Instance dec_eq_tree : Dec_Eq Tree.
+Proof. dec_eq. Defined.
+    
+
+Axiom number_of_trials : nat.
+Extract Constant number_of_trials => "20000".
+
+
+(* --------------------- Tests --------------------- *)
+
+Definition test_prop_InsertValid   :=
+	@ForAll _ ∅ _ "t" (fun tt => arbitrary) (fun tt n => (fun n => arbitrary)) (fun tt n => shrink n) (fun tt n => show n) (
+	@ForAll _ (Tree · ∅) _ "k" (fun '(t, tt) => arbitrary) (fun '(t, tt) n => (fun n => arbitrary)) (fun '(t, tt) n => shrink n) (fun '(t, tt) n => show n) (
+	@ForAll _ (Z · (Tree · ∅)) _ "v" (fun '(k, (t, tt)) => arbitrary) (fun '(k, (t, tt)) n => (fun n => arbitrary)) (fun '(k, (t, tt)) n => shrink n) (fun '(k, (t, tt)) n => show n) (
+	@Predicate (Z · (Z · (Tree · ∅))) Z
+	(fun '(v, (k, (t, tt))) => (prop_InsertValid t k v, 0%Z))))).
+
+Definition test_prop_InsertValid_runner := (targetLoop number_of_trials test_prop_InsertValid (DynamicResettingSingletonPool.(mkPool) tt) DynamicResettingSingletonPool HillClimbingUtility).
+
+(*! QuickProp test_prop_InsertValid_runner. *)
+
+Definition test_prop_DeleteValid   :=
+	@ForAll _ ∅ _ "t" (fun tt => arbitrary) (fun tt n => (fun n => arbitrary)) (fun tt n => shrink n) (fun tt n => show n) (
+	@ForAll _ (Tree · ∅) _ "k" (fun '(t, tt) => arbitrary) (fun '(t, tt) n => (fun n => arbitrary)) (fun '(t, tt) n => shrink n) (fun '(t, tt) n => show n) (
+	@Predicate (Z · (Tree · ∅)) Z
+	(fun '(k, (t, tt)) => (prop_DeleteValid t k, 0%Z)))).
+
+Definition test_prop_DeleteValid_runner := (targetLoop number_of_trials test_prop_DeleteValid (DynamicResettingSingletonPool.(mkPool) tt) DynamicResettingSingletonPool HillClimbingUtility).
+
+(*! QuickProp test_prop_DeleteValid_runner. *)
+
+Definition test_prop_InsertPost    :=
+	@ForAll _ ∅ _ "t" (fun tt => arbitrary) (fun tt n => (fun n => arbitrary)) (fun tt n => shrink n) (fun tt n => show n) (
+	@ForAll _ (Tree · ∅) _ "k" (fun '(t, tt) => arbitrary) (fun '(t, tt) n => (fun n => arbitrary)) (fun '(t, tt) n => shrink n) (fun '(t, tt) n => show n) (
+	@ForAll _ (Z · (Tree · ∅)) _ "k'" (fun '(k, (t, tt)) => arbitrary) (fun '(k, (t, tt)) n => (fun n => arbitrary)) (fun '(k, (t, tt)) n => shrink n) (fun '(k, (t, tt)) n => show n) (
+	@ForAll _ (Z · (Z · (Tree · ∅))) _ "v" (fun '(k', (k, (t, tt))) => arbitrary) (fun '(k', (k, (t, tt))) n => (fun n => arbitrary)) (fun '(k', (k, (t, tt))) n => shrink n) (fun '(k', (k, (t, tt))) n => show n) (
+	@Predicate (Z · (Z · (Z · (Tree · ∅)))) Z
+	(fun '(v, (k', (k, (t, tt)))) => (prop_InsertPost t k k' v, 0%Z)))))).
+
+Definition test_prop_InsertPost_runner := (targetLoop number_of_trials test_prop_InsertPost (DynamicResettingSingletonPool.(mkPool) tt) DynamicResettingSingletonPool HillClimbingUtility).
+(*! QuickProp test_prop_InsertPost_runner. *)
+
+Definition test_prop_DeletePost    :=
+	@ForAll _ ∅ _ "t" (fun tt => arbitrary) (fun tt n => (fun n => arbitrary)) (fun tt n => shrink n) (fun tt n => show n) (
+	@ForAll _ (Tree · ∅) _ "k" (fun '(t, tt) => arbitrary) (fun '(t, tt) n => (fun n => arbitrary)) (fun '(t, tt) n => shrink n) (fun '(t, tt) n => show n) (
+	@ForAll _ (Z · (Tree · ∅)) _ "k'" (fun '(k, (t, tt)) => arbitrary) (fun '(k, (t, tt)) n => (fun n => arbitrary)) (fun '(k, (t, tt)) n => shrink n) (fun '(k, (t, tt)) n => show n) (
+	@Predicate (Z · (Z · (Tree · ∅))) Z
+	(fun '(k', (k, (t, tt))) => (prop_DeletePost t k k', 0%Z))))).
+
+Definition test_prop_DeletePost_runner := (targetLoop number_of_trials test_prop_DeletePost (DynamicResettingSingletonPool.(mkPool) tt) DynamicResettingSingletonPool HillClimbingUtility).
+(*! QuickProp test_prop_DeletePost_runner. *)
+
+Definition test_prop_InsertModel    :=
+	@ForAll _ ∅ _ "t" (fun tt => arbitrary) (fun tt n => (fun n => arbitrary)) (fun tt n => shrink n) (fun tt n => show n) (
+	@ForAll _ (Tree · ∅) _ "k" (fun '(t, tt) => arbitrary) (fun '(t, tt) n => (fun n => arbitrary)) (fun '(t, tt) n => shrink n) (fun '(t, tt) n => show n) (
+	@ForAll _ (Z · (Tree · ∅)) _ "v'" (fun '(v, (t, tt)) => arbitrary) (fun '(v, (t, tt)) n => (fun n => arbitrary)) (fun '(v, (t, tt)) n => shrink n) (fun '(v, (t, tt)) n => show n) (
+	@Predicate (Z · (Z · (Tree · ∅))) Z
+	(fun '(v, (k, (t, tt))) => (prop_InsertModel t k v, 0%Z))))).
+
+    
+Definition test_prop_InsertModel_runner := (targetLoop number_of_trials test_prop_InsertModel (DynamicResettingSingletonPool.(mkPool) tt) DynamicResettingSingletonPool HillClimbingUtility).
+(*! QuickProp test_prop_InsertModel_runner. *)
+
+Definition test_prop_DeleteModel    :=
+	@ForAll _ ∅ _ "t" (fun tt => arbitrary) (fun tt n => (fun n => arbitrary)) (fun tt n => shrink n) (fun tt n => show n) (
+	@ForAll _ (Tree · ∅) _ "k" (fun '(t, tt) => arbitrary) (fun '(t, tt) n => (fun n => arbitrary)) (fun '(t, tt) n => shrink n) (fun '(t, tt) n => show n) (
+	@Predicate (Z · (Tree · ∅)) Z
+	(fun '(k, (t, tt)) => (prop_DeleteModel t k, 0%Z)))).
+
+    
+Definition test_prop_DeleteModel_runner := (targetLoop number_of_trials test_prop_DeleteModel (DynamicResettingSingletonPool.(mkPool) tt) DynamicResettingSingletonPool HillClimbingUtility).
+(*! QuickProp test_prop_DeleteModel_runner. *)
+
+Definition test_prop_InsertInsert    :=
+	@ForAll _ ∅ _ "t" (fun tt => arbitrary) (fun tt n => (fun n => arbitrary)) (fun tt n => shrink n) (fun tt n => show n) (
+	@ForAll _ (Tree · ∅) _ "k" (fun '(t, tt) => arbitrary) (fun '(t, tt) n => (fun n => arbitrary)) (fun '(t, tt) n => shrink n) (fun '(t, tt) n => show n) (
+	@ForAll _ (Z · (Tree · ∅)) _ "k'" (fun '(k, (t, tt)) => arbitrary) (fun '(k, (t, tt)) n => (fun n => arbitrary)) (fun '(k, (t, tt)) n => shrink n) (fun '(k, (t, tt)) n => show n) (
+	@ForAll _ (Z · (Z · (Tree · ∅))) _ "v" (fun '(k', (k, (t, tt))) => arbitrary) (fun '(k', (k, (t, tt))) n => (fun n => arbitrary)) (fun '(k', (k, (t, tt))) n => shrink n) (fun '(k', (k, (t, tt))) n => show n) (
+	@ForAll _ (Z · (Z · (Z · (Tree · ∅)))) _ "v'" (fun '(v, (k', (k, (t, tt)))) => arbitrary) (fun '(v, (k', (k, (t, tt)))) n => (fun n => arbitrary)) (fun '(v, (k', (k, (t, tt)))) n => shrink n) (fun '(v, (k', (k, (t, tt)))) n => show n) (
+	@Predicate (Z · (Z · (Z · (Z · (Tree · ∅))))) Z
+	(fun '(v', (v, (k', (k, (t, tt))))) => (prop_InsertInsert t k k' v v', 0%Z))))))).
+
+Definition test_prop_InsertInsert_runner := (targetLoop number_of_trials test_prop_InsertInsert (DynamicResettingSingletonPool.(mkPool) tt) DynamicResettingSingletonPool HillClimbingUtility).
+(*! QuickProp test_prop_InsertInsert_runner. *)
+
+Definition test_prop_InsertDelete    :=
+	@ForAll _ ∅ _ "t" (fun tt => arbitrary) (fun tt n => (fun n => arbitrary)) (fun tt n => shrink n) (fun tt n => show n) (
+	@ForAll _ (Tree · ∅) _ "k" (fun '(t, tt) => arbitrary) (fun '(t, tt) n => (fun n => arbitrary)) (fun '(t, tt) n => shrink n) (fun '(t, tt) n => show n) (
+	@ForAll _ (Z · (Tree · ∅)) _ "k'" (fun '(k, (t, tt)) => arbitrary) (fun '(k, (t, tt)) n => (fun n => arbitrary)) (fun '(k, (t, tt)) n => shrink n) (fun '(k, (t, tt)) n => show n) (
+	@ForAll _ (Z · (Z · (Tree · ∅))) _ "v" (fun '(k', (k, (t, tt))) => arbitrary) (fun '(k', (k, (t, tt))) n => (fun n => arbitrary)) (fun '(k', (k, (t, tt))) n => shrink n) (fun '(k', (k, (t, tt))) n => show n) (
+	@Predicate (Z · (Z · (Z · (Tree · ∅)))) Z
+	(fun '(v, (k', (k, (t, tt)))) => (prop_InsertDelete t k k' v, 0%Z)))))).
+
+Definition test_prop_InsertDelete_runner := (targetLoop number_of_trials test_prop_InsertDelete (DynamicResettingSingletonPool.(mkPool) tt) DynamicResettingSingletonPool HillClimbingUtility).
+(*! QuickProp test_prop_InsertDelete_runner. *)
+
+
+Definition test_prop_DeleteInsert    :=
+	@ForAll _ ∅ _ "t" (fun tt => arbitrary) (fun tt n => (fun n => arbitrary)) (fun tt n => shrink n) (fun tt n => show n) (
+	@ForAll _ (Tree · ∅) _ "k" (fun '(t, tt) => arbitrary) (fun '(t, tt) n => (fun n => arbitrary)) (fun '(t, tt) n => shrink n) (fun '(t, tt) n => show n) (
+	@ForAll _ (Z · (Tree · ∅)) _ "k'" (fun '(k, (t, tt)) => arbitrary) (fun '(k, (t, tt)) n => (fun n => arbitrary)) (fun '(k, (t, tt)) n => shrink n) (fun '(k, (t, tt)) n => show n) (
+	@ForAll _ (Z · (Z · (Tree · ∅))) _ "v'" (fun '(k', (k, (t, tt))) => arbitrary) (fun '(k', (k, (t, tt))) n => (fun n => arbitrary)) (fun '(k', (k, (t, tt))) n => shrink n) (fun '(k', (k, (t, tt))) n => show n) (
+	@Predicate (Z · (Z · (Z · (Tree · ∅)))) Z
+	(fun '(v', (k', (k, (t, tt)))) => (prop_DeleteInsert t k k' v', 0%Z)))))).
+
+Definition test_prop_DeleteInsert_runner := (targetLoop number_of_trials test_prop_DeleteInsert (DynamicResettingSingletonPool.(mkPool) tt) DynamicResettingSingletonPool HillClimbingUtility).
+(*! QuickProp test_prop_DeleteInsert_runner. *)
+
+Definition test_prop_DeleteDelete    :=
+	@ForAll _ ∅ _ "t" (fun tt => arbitrary) (fun tt n => (fun n => arbitrary)) (fun tt n => shrink n) (fun tt n => show n) (
+	@ForAll _ (Tree · ∅) _ "k" (fun '(t, tt) => arbitrary) (fun '(t, tt) n => (fun n => arbitrary)) (fun '(t, tt) n => shrink n) (fun '(t, tt) n => show n) (
+	@ForAll _ (Z · (Tree · ∅)) _ "k'" (fun '(k, (t, tt)) => arbitrary) (fun '(k, (t, tt)) n => (fun n => arbitrary)) (fun '(k, (t, tt)) n => shrink n) (fun '(k, (t, tt)) n => show n) (
+	@Predicate (Z · (Z · (Tree · ∅))) Z
+	(fun '(k', (k, (t, tt))) => ((prop_DeleteDelete t k k', 0%Z)))))).
+
+Definition test_prop_DeleteDelete_runner := (targetLoop number_of_trials test_prop_DeleteDelete (DynamicResettingSingletonPool.(mkPool) tt) DynamicResettingSingletonPool HillClimbingUtility).
+(*! QuickProp test_prop_DeleteDelete_runner. *)
